verify/Inductive.v
@@ -1,0 +1,3477 @@
+From BusyCoq Require Import Individual.
+Require Import List.
+Require Import ZArith.
+Require Import Lia.
+Require Import FSets.FMapPositive.
+
+Notation "x || y" := (if x then true else y) : bool_scope.
+Notation "x && y" := (if x then y else false) : bool_scope.
+Open Scope bool.
+
+Lemma or_false_iff (a b:bool):
+  (a || b) = false <->
+  a = false /\ b = false.
+Proof.
+  destruct a,b; tauto.
+Qed.
+
+Lemma and_true_iff (a b:bool):
+  (a && b) = true <->
+  a = true /\ b = true.
+Proof.
+  destruct a,b; tauto.
+Qed.
+
+
+
+
+Ltac destruct_spec_expr e f :=
+match e with
+| match ?a with _ => _ end => destruct_spec_expr a f
+| if ?a then _ else _ => destruct_spec_expr a f
+| ?a ?arg1 ?arg2 ?arg3 ?arg4 ?arg5 =>
+  pose proof (f arg1 arg2 arg3 arg4 arg5);
+  destruct e
+| ?a ?arg1 ?arg2 ?arg3 ?arg4 =>
+  pose proof (f arg1 arg2 arg3 arg4);
+  destruct e
+| ?a ?arg1 ?arg2 ?arg3 =>
+  pose proof (f arg1 arg2 arg3);
+  destruct e
+| ?a ?arg1 ?arg2 =>
+  pose proof (f arg1 arg2);
+  destruct e
+| ?a ?arg1 =>
+  pose proof (f arg1);
+  destruct e
+end.
+
+Ltac destruct_spec f :=
+match goal with
+|- ?a => destruct_spec_expr a f
+end.
+
+
+
+
+
+Fixpoint exgcdn(n:nat)(a b:Z):Z*Z :=
+(match n with
+| O => (1,0)
+| S n0 =>
+  match b with
+  | Z0 => (1,0)
+  | _ =>
+    let (y,x):=exgcdn n0 b (a mod b) in
+    (x,y-a/b*x)
+  end
+end)%Z.
+
+Definition N_to_Pos(x:N):=
+match x with
+| N0 => xH
+| Npos x0 => x0
+end.
+
+Definition exgcd(a b:N):N*N :=
+  let (x,y):=
+  exgcdn ((Nat.max (Pos.size_nat (N_to_Pos a)) (Pos.size_nat (N_to_Pos b)))*2) (Z.of_N a) (Z.of_N b) in
+  (Z.to_N (if x <? 0 then (x+Z.of_N b) else x),Z.to_N (if y <? 0 then (y+Z.of_N a) else y))%Z.
+
+
+
+
+
+Module Inductive(Ctx:Ctx).
+
+Module TM := TM Ctx. Export TM.
+
+Definition multistep' tm (p:bool) s0 s1 :=
+if p then s0-[tm]->+s1 else s0-[tm]->*s1.
+
+
+Definition id_t := positive.
+
+Inductive type_t :=
+| nat_t
+| seg_t
+| side_t
+.
+
+Definition to_type(x:type_t):Type :=
+match x with
+| nat_t => N
+| seg_t => list Sym
+| side_t => side
+end.
+
+
+Inductive nat_expr :=
+| from_nat(n:N)
+| nat_add(a b:nat_expr)
+| nat_mul(a b:nat_expr)
+| nat_var(i:id_t)
+| nat_ivar
+.
+
+Inductive seg_expr :=
+| seg_sym(a:Sym)
+| seg_concat(a:seg_expr)(b:seg_expr)
+| seg_repeat(a:seg_expr)(n:nat_expr)
+| seg_var(i:id_t)
+.
+
+Inductive side_expr :=
+| side_0inf
+| side_var(i:id_t)
+| side_concat(a:seg_expr)(b:side_expr)
+.
+
+Definition to_expr_type(x:type_t):Type :=
+match x with
+| nat_t => nat_expr
+| seg_t => seg_expr
+| side_t => side_expr
+end.
+
+Definition expr_expr := {x:type_t & to_expr_type x}.
+Definition make_expr_expr(t:type_t)(x:to_expr_type t):expr_expr.
+  exists t.
+  apply x.
+Defined.
+
+
+Definition config_expr:Type := side_expr*side_expr*Q*dir.
+
+Inductive prop0_expr :=
+| nat_eq(a b:nat_expr)
+| seg_eq(a b:seg_expr)
+| side_eq(a b:side_expr)
+| config_eq(a b:config_expr)
+| false_prop0
+| multistep_expr(a b:config_expr)(n:nat_expr)
+| multistep'_expr(a b:config_expr)(n:bool)
+.
+
+Definition prop_expr:Type :=
+  (list prop0_expr)*(list prop0_expr).
+
+
+
+Fixpoint nat_expr_eqb(a b:nat_expr):bool :=
+match a,b with
+| from_nat a0,from_nat b0 => (a0 =? b0)%N
+| nat_add a0 a1,nat_add b0 b1 => (nat_expr_eqb a0 b0) && (nat_expr_eqb a1 b1)
+| nat_mul a0 a1,nat_mul b0 b1 => (nat_expr_eqb a0 b0) && (nat_expr_eqb a1 b1)
+| nat_var a0,nat_var b0 => (a0 =? b0)%positive
+| nat_ivar,nat_ivar => true
+| _,_ => false
+end.
+
+Ltac solve_Bool_reflect :=
+  try (constructor; congruence).
+
+Lemma nat_expr_eqb_spec(a b:nat_expr): Bool.reflect (a=b) (nat_expr_eqb a b).
+Proof.
+  gen b.
+  induction a; intros b; destruct b; cbn.
+  all: solve_Bool_reflect.
+  - destruct (N.eqb_spec n n0);
+    solve_Bool_reflect.
+  - destruct (IHa1 b1),(IHa2 b2); subst; cbn;
+    solve_Bool_reflect.
+  - destruct (IHa1 b1),(IHa2 b2); subst; cbn;
+    solve_Bool_reflect.
+  - destruct (Pos.eqb_spec i i0);
+    solve_Bool_reflect.
+Qed.
+
+Fixpoint seg_expr_eqb(a b:seg_expr):bool :=
+match a,b with
+| seg_sym a0,seg_sym b0 => sym_eqb a0 b0
+| seg_concat a0 a1,seg_concat b0 b1 => seg_expr_eqb a0 b0 && seg_expr_eqb a1 b1
+| seg_repeat a0 an,seg_repeat b0 bn => seg_expr_eqb a0 b0 && nat_expr_eqb an bn
+| seg_var a0,seg_var b0 => (a0 =? b0)%positive
+| _,_ => false
+end.
+
+Lemma seg_expr_eqb_spec(a b:seg_expr): Bool.reflect (a=b) (seg_expr_eqb a b).
+Proof.
+  gen b.
+  induction a; intros b; destruct b; cbn.
+  all: solve_Bool_reflect.
+  - destruct (sym_eqb_spec a a0);
+    solve_Bool_reflect.
+  - destruct (IHa1 b1),(IHa2 b2); subst; cbn;
+    solve_Bool_reflect.
+  - destruct (IHa b),(nat_expr_eqb_spec n n0); subst; cbn;
+    solve_Bool_reflect.
+  - destruct (Pos.eqb_spec i i0);
+    solve_Bool_reflect.
+Qed.
+
+Fixpoint side_expr_eqb(a b:side_expr):bool :=
+match a,b with
+| side_0inf,side_0inf => true
+| side_var a0,side_var b0 => (a0 =? b0)%positive
+| side_concat a0 a1,side_concat b0 b1 => seg_expr_eqb a0 b0 && side_expr_eqb a1 b1
+| _,_ => false
+end.
+
+Lemma side_expr_eqb_spec(a b:side_expr): Bool.reflect (a=b) (side_expr_eqb a b).
+Proof.
+  gen b.
+  induction a; intros b; destruct b; cbn.
+  all: solve_Bool_reflect.
+  - destruct (Pos.eqb_spec i i0);
+    solve_Bool_reflect.
+  - destruct (IHa b),(seg_expr_eqb_spec a a1); subst; cbn;
+    solve_Bool_reflect.
+Qed.
+
+Definition dir_eqb(a b:dir):bool :=
+match a,b with
+| L,L | R,R => true
+| _,_ => false
+end.
+
+Lemma dir_eqb_spec(a b:dir): Bool.reflect (a=b) (dir_eqb a b).
+Proof.
+  destruct a,b;
+  solve_Bool_reflect.
+Qed.
+
+Definition config_expr_eqb(a b:config_expr):bool :=
+let '(l1,r1,s1,sgn1) := a in
+let '(l2,r2,s2,sgn2) := b in
+(q_eqb s1 s2) && (dir_eqb sgn1 sgn2) &&
+(side_expr_eqb l1 l2) && (side_expr_eqb r1 r2).
+
+Lemma config_expr_eqb_spec(a b:config_expr): Bool.reflect (a=b) (config_expr_eqb a b).
+Proof.
+  destruct a as [[[l1 r1] s1] sgn1].
+  destruct b as [[[l2 r2] s2] sgn2].
+  cbn.
+  destruct (q_eqb_spec s1 s2); solve_Bool_reflect.
+  destruct (dir_eqb_spec sgn1 sgn2); solve_Bool_reflect.
+  destruct (side_expr_eqb_spec l1 l2); solve_Bool_reflect.
+  destruct (side_expr_eqb_spec r1 r2); solve_Bool_reflect.
+Qed.
+
+Definition prop0_eqb(a b:prop0_expr):bool :=
+match a,b with
+| nat_eq a0 a1,nat_eq b0 b1 => nat_expr_eqb a0 b0 && nat_expr_eqb a1 b1
+| seg_eq a0 a1,seg_eq b0 b1 => seg_expr_eqb a0 b0 && seg_expr_eqb a1 b1
+| side_eq a0 a1,side_eq b0 b1 => side_expr_eqb a0 b0 && side_expr_eqb a1 b1
+| config_eq a0 a1,config_eq b0 b1 => config_expr_eqb a0 b0 && config_expr_eqb a1 b1
+| false_prop0,false_prop0 => true
+| multistep_expr a0 a1 an,multistep_expr b0 b1 bn =>
+  config_expr_eqb a0 b0 && config_expr_eqb a1 b1 && nat_expr_eqb an bn
+| multistep'_expr a0 a1 an,multistep'_expr b0 b1 bn =>
+  config_expr_eqb a0 b0 && config_expr_eqb a1 b1 && Bool.eqb an bn
+| _,_ => false
+end.
+
+Lemma prop0_eqb_spec a b: Bool.reflect (a=b) (prop0_eqb a b).
+Proof.
+  destruct a,b; cbn; solve_Bool_reflect.
+  - destruct (nat_expr_eqb_spec a a0); solve_Bool_reflect.
+    destruct (nat_expr_eqb_spec b0 b); solve_Bool_reflect.
+  - destruct (seg_expr_eqb_spec a a0); solve_Bool_reflect.
+    destruct (seg_expr_eqb_spec b0 b); solve_Bool_reflect.
+  - destruct (side_expr_eqb_spec a a0); solve_Bool_reflect.
+    destruct (side_expr_eqb_spec b0 b); solve_Bool_reflect.
+  - destruct (config_expr_eqb_spec a a0); solve_Bool_reflect.
+    destruct (config_expr_eqb_spec b0 b); solve_Bool_reflect.
+  - destruct (config_expr_eqb_spec a a0); solve_Bool_reflect.
+    destruct (config_expr_eqb_spec b0 b); solve_Bool_reflect.
+    destruct (nat_expr_eqb_spec n n0); solve_Bool_reflect.
+  - destruct (config_expr_eqb_spec a a0); solve_Bool_reflect.
+    destruct (config_expr_eqb_spec b0 b); solve_Bool_reflect.
+    destruct (Bool.eqb_spec n n0); solve_Bool_reflect.
+Qed.
+
+Fixpoint list_prop0_eqb(a b:list prop0_expr):bool :=
+match a,b with
+| nil,nil => true
+| a0::a1,b0::b1 =>
+  prop0_eqb a0 b0 &&
+  list_prop0_eqb a1 b1
+| _,_ => false
+end.
+
+Lemma list_prop0_eqb_spec a b: Bool.reflect (a=b) (list_prop0_eqb a b).
+Proof.
+  gen b.
+  induction a; destruct b; cbn; solve_Bool_reflect.
+  - specialize (IHa b).
+    destruct (prop0_eqb_spec a p); solve_Bool_reflect.
+    destruct IHa; solve_Bool_reflect.
+Qed.
+
+Definition prop_eqb(a b:prop_expr):bool :=
+let (a0,a1):=a in
+let (b0,b1):=b in
+list_prop0_eqb a0 b0 &&
+list_prop0_eqb a1 b1.
+
+Lemma prop_eqb_spec a b: Bool.reflect (a=b) (prop_eqb a b).
+Proof.
+  destruct a as [a0 a1].
+  destruct b as [b0 b1].
+  cbn.
+  destruct (list_prop0_eqb_spec a0 b0); solve_Bool_reflect.
+  destruct (list_prop0_eqb_spec a1 b1); solve_Bool_reflect.
+Qed.
+
+
+
+Definition affine_map := list (nat_expr*Z).
+Fixpoint affine_map_upd'(f:affine_map)(x:nat_expr)(u:Z):affine_map*bool :=
+match f with
+| nil => (nil,false)
+| (x0,y0)::f1 =>
+  if nat_expr_eqb x0 x then
+    ((x0,(y0+u)%Z)::f1,true)
+  else
+    let '(f2,t):=affine_map_upd' f1 x u in
+    ((x0,y0)::f2,t)
+end.
+
+Definition affine_map_upd(f:affine_map)(x:nat_expr)(u:Z):affine_map :=
+let '(f1,t):=affine_map_upd' f x u in
+if t then f1 else (x,u)::f1.
+
+
+Fixpoint from_affine_map(f:affine_map):nat_expr*nat_expr :=
+match f with
+| nil => (from_nat 0,from_nat 0)
+| (x0,y0)::f0 =>
+  let (v1,v2):=from_affine_map f0 in
+  match y0 with
+  | Zpos y1 => (nat_add v1 (nat_mul x0 (from_nat (Npos y1))),v2)
+  | Zneg y1 => (v1,nat_add v2 (nat_mul x0 (from_nat (Npos y1))))
+  | Z0 => (v1,v2)
+  end
+end.
+
+Fixpoint affine_map_gcd(f:affine_map):Z :=
+match f with
+| nil => Z0
+| (x0,y0)::f1 =>
+  let g := affine_map_gcd f1 in
+  if nat_expr_eqb x0 (from_nat 1) then g else (Z.gcd g y0)
+end.
+
+Fixpoint affine_map_divide(f:affine_map)(g:Z):Prop :=
+match f with
+| nil => True
+| (x0,y0)::f1 =>
+  (if nat_expr_eqb x0 (from_nat 1) then True else (Z.divide g y0)) /\
+  (affine_map_divide f1 g)
+end.
+
+Lemma affine_map_divide_trans f g0 g1:
+  Z.divide g1 g0 ->
+  affine_map_divide f g0 ->
+  affine_map_divide f g1.
+Proof.
+  intros H.
+  induction f as [|[x0 y0] f]; intros; cbn.
+  1: trivial.
+  cbn in H0.
+  destruct (nat_expr_eqb_spec x0 (from_nat 1)).
+  1: tauto.
+  split. 2: tauto.
+  eapply Z.divide_trans; eauto; tauto.
+Qed.
+
+Lemma affine_map_gcd_spec f:
+  affine_map_divide f (affine_map_gcd f).
+Proof.
+  induction f as [|[x0 y0] f]; cbn.
+  1: trivial.
+  destruct (nat_expr_eqb_spec x0 (from_nat 1)).
+  1: tauto.
+  remember (affine_map_gcd f) as g.
+  pose proof (Z.gcd_divide_l g y0) as H.
+  pose proof (Z.gcd_divide_r g y0) as H0.
+  split. 1: tauto.
+  clear H0.
+  eapply affine_map_divide_trans; eauto.
+Qed.
+
+Fixpoint affine_map_div(f:affine_map)(g:Z):(affine_map*Z) :=
+match f with
+| nil => (nil,Z0)
+| (x0,y0)::f1 =>
+  let (f2,m2) := affine_map_div f1 g in
+  ((x0,y0/g)::f2,(if nat_expr_eqb x0 (from_nat 1) then (m2+(y0 mod g)) else m2))%Z
+end.
+
+Fixpoint add_to_affine_map(a:nat_expr)(sgn:Z)(f:affine_map):affine_map :=
+match a with
+| nat_add a0 a1 =>
+  let f0 := add_to_affine_map a0 sgn f in
+  add_to_affine_map a1 sgn f0
+| nat_mul a0 (from_nat a1) =>
+  add_to_affine_map a0 (sgn*(Z.of_N a1))%Z f
+| from_nat a1 => affine_map_upd f (from_nat 1) (sgn*(Z.of_N a1))%Z
+| _ => affine_map_upd f a sgn
+end.
+
+
+
+
+Definition simpl_nat_expr(x:nat_expr) :=
+match x with
+| nat_add (from_nat 0) b => b
+| nat_add (from_nat a) b => nat_add b (from_nat a)
+| nat_add (nat_add a (from_nat b)) c => nat_add (nat_add a c) (from_nat b)
+| nat_mul (from_nat 1) b => b
+| nat_mul b (from_nat 1) => b
+| _ => x
+end.
+
+Fixpoint simpls_nat_expr(x:nat_expr) :=
+match x with
+| nat_add a b => simpl_nat_expr (nat_add (simpls_nat_expr a) (simpls_nat_expr b))
+| nat_mul a b => simpl_nat_expr (nat_mul (simpls_nat_expr a) (simpls_nat_expr b))
+| _ => x
+end.
+
+Definition simpl_nat_expr_by_affine_map(a:nat_expr) :=
+let f := add_to_affine_map a 1 nil in
+let (v1,v2) := from_affine_map f in
+if nat_expr_eqb v2 (from_nat 0) then v1 else a.
+
+
+Definition list_prop0_from_affine_map f :=
+let (v1,v2) := from_affine_map f in
+if nat_expr_eqb v1 v2 then [] else [nat_eq (simpls_nat_expr v1) (simpls_nat_expr v2)].
+
+Definition from_affine_map_simpl_div(f:affine_map):list prop0_expr :=
+let g := affine_map_gcd f in
+if (1 <? g)%Z then
+  let (f0,g0) := affine_map_div f g in
+  if (g0 =? 0)%Z then list_prop0_from_affine_map f0
+  else if (g0 mod g =? 0)%Z then list_prop0_from_affine_map f
+  else [false_prop0]
+else list_prop0_from_affine_map f.
+
+
+
+Definition solve_nat_eq(a b:nat_expr):list prop0_expr :=
+let f := add_to_affine_map a 1 nil in
+let f0 := add_to_affine_map b (-1) f in
+from_affine_map_simpl_div f0.
+
+Fixpoint solve_seg_eq(a b:seg_expr):list prop0_expr :=
+match a,b with
+| seg_sym a0,seg_sym b0 => if sym_eqb a0 b0 then [] else [false_prop0]
+| seg_concat a0 a1,seg_concat b0 b1 => (solve_seg_eq a0 b0) ++ (solve_seg_eq a1 b1)
+| seg_repeat a0 a1,seg_repeat b0 b1 => (solve_seg_eq a0 b0) ++ (solve_nat_eq a1 b1)
+| seg_var a0,seg_var b0 => if (a0=?b0)%positive then [] else [seg_eq a b]
+| _,_ => [seg_eq a b]
+end.
+
+Fixpoint solve_side_eq(a b:side_expr):list prop0_expr :=
+match a,b with
+| side_0inf,side_0inf => []
+| side_var a0,side_var b0 => if (a0=?b0)%positive then [] else [side_eq a b]
+| side_concat a0 a1,side_concat b0 b1 => (solve_seg_eq a0 b0) ++ (solve_side_eq a1 b1)
+| _,_ => [side_eq a b]
+end.
+
+Definition solve_config_eq(a b:config_expr):list prop0_expr :=
+let '(l1,r1,s1,d1):=a in
+let '(l2,r2,s2,d2):=b in
+(if q_eqb s1 s2 && dir_eqb d1 d2 then (solve_side_eq l1 l2) ++ (solve_side_eq r1 r2) else [false_prop0]).
+
+Definition solve_eq(x:prop0_expr):list prop0_expr :=
+match x with
+| nat_eq a b => solve_nat_eq a b
+| seg_eq a b => solve_seg_eq a b
+| side_eq a b => solve_side_eq a b
+| config_eq a b => solve_config_eq a b
+| _ => [x]
+end.
+
+Definition solve_eqs x :=
+  flat_map solve_eq x.
+
+Definition prop_solve_eq(x:prop_expr) :=
+let (H,G):=x in (solve_eqs H,G).
+
+Fixpoint has_false(x:list prop0_expr) :=
+match x with
+| nil => false
+| false_prop0::t => true
+| _::t => has_false t
+end.
+
+Definition prop_has_false(x:prop_expr) :=
+let (H,G):=x in has_false H.
+
+
+
+
+(*
+  syntatic equality (but nat_expr are compared using affine_map)
+*)
+Module ExprEq.
+
+Definition nat_expr_eqb(a b:nat_expr):bool :=
+match solve_nat_eq a b with
+| nil => true
+| _ => false
+end.
+
+Fixpoint seg_expr_eqb(a b:seg_expr):bool :=
+match a,b with
+| seg_sym a0,seg_sym b0 => sym_eqb a0 b0
+| seg_concat a0 a1,seg_concat b0 b1 => seg_expr_eqb a0 b0 && seg_expr_eqb a1 b1
+| seg_repeat a0 an,seg_repeat b0 bn => seg_expr_eqb a0 b0 && nat_expr_eqb an bn
+| seg_var a0,seg_var b0 => (a0 =? b0)%positive
+| _,_ => false
+end.
+
+Fixpoint side_expr_eqb(a b:side_expr):bool :=
+match a,b with
+| side_0inf,side_0inf => true
+| side_var a0,side_var b0 => (a0 =? b0)%positive
+| side_concat a0 a1,side_concat b0 b1 => seg_expr_eqb a0 b0 && side_expr_eqb a1 b1
+| _,_ => false
+end.
+
+Definition config_expr_eqb(a b:config_expr):bool :=
+let '(l1,r1,s1,sgn1) := a in
+let '(l2,r2,s2,sgn2) := b in
+(q_eqb s1 s2) && (dir_eqb sgn1 sgn2) &&
+(side_expr_eqb l1 l2) && (side_expr_eqb r1 r2).
+
+Definition prop0_eqb(a b:prop0_expr):bool :=
+match a,b with
+| nat_eq a0 a1,nat_eq b0 b1 => nat_expr_eqb a0 b0 && nat_expr_eqb a1 b1
+| seg_eq a0 a1,seg_eq b0 b1 => seg_expr_eqb a0 b0 && seg_expr_eqb a1 b1
+| side_eq a0 a1,side_eq b0 b1 => side_expr_eqb a0 b0 && side_expr_eqb a1 b1
+| config_eq a0 a1,config_eq b0 b1 => config_expr_eqb a0 b0 && config_expr_eqb a1 b1
+| false_prop0,false_prop0 => true
+| multistep_expr a0 a1 an,multistep_expr b0 b1 bn =>
+  config_expr_eqb a0 b0 && config_expr_eqb a1 b1 && nat_expr_eqb an bn
+| multistep'_expr a0 a1 an,multistep'_expr b0 b1 bn =>
+  config_expr_eqb a0 b0 && config_expr_eqb a1 b1 && Bool.eqb an bn
+| _,_ => false
+end.
+
+Fixpoint list_prop0_eqb(a b:list prop0_expr):bool :=
+match a,b with
+| nil,nil => true
+| a0::a1,b0::b1 =>
+  prop0_eqb a0 b0 &&
+  list_prop0_eqb a1 b1
+| _,_ => false
+end.
+
+Definition prop_eqb(a b:prop_expr):bool :=
+let (a0,a1):=a in
+let (b0,b1):=b in
+list_prop0_eqb a0 b0 &&
+list_prop0_eqb a1 b1.
+
+End ExprEq.
+
+
+
+Section allFV.
+
+Definition S:Type := (PositiveMap.tree id_t)*positive.
+Definition S0 := (PositiveMap.empty id_t,xH).
+Definition add_var(s:S)(i:id_t):S :=
+let (f,p):=s in
+match PositiveMap.find i f with
+| None => (PositiveMap.add i p f,Pos.succ p)
+| Some _ => s
+end.
+
+Fixpoint nat_allFV(x:nat_expr)(s:S):S :=
+match x with
+| from_nat x0 => s
+| nat_add a b => nat_allFV a (nat_allFV b s)
+| nat_mul a b => nat_allFV a (nat_allFV b s)
+| nat_var i0 => add_var s i0
+| nat_ivar => s
+end.
+
+Fixpoint seg_allFV(x:seg_expr)(s:S):S :=
+match x with
+| seg_sym a => s
+| seg_concat a b => seg_allFV a (seg_allFV b s)
+| seg_repeat a n => seg_allFV a (nat_allFV n s)
+| seg_var i0 => add_var s i0
+end.
+
+Fixpoint side_allFV(x:side_expr)(s:S):S :=
+match x with
+| side_0inf => s
+| side_var i0 => add_var s i0
+| side_concat a b => seg_allFV a (side_allFV b s)
+end.
+
+
+Definition expr_allFV(e:expr_expr):=
+match e with
+| existT _ nat_t x => nat_allFV x
+| existT _ seg_t x => seg_allFV x
+| existT _ side_t x => side_allFV x
+end.
+
+
+Definition config_allFV(x:config_expr)(s:S):S :=
+  let '(l,r,_,_):=x in
+  side_allFV l (side_allFV r s).
+
+Definition prop0_allFV(x:prop0_expr)(s:S):S :=
+match x with
+| nat_eq a b => nat_allFV b (nat_allFV a s)
+| seg_eq a b => seg_allFV b (seg_allFV a s)
+| side_eq a b => side_allFV b (side_allFV a s)
+| config_eq a b => config_allFV b (config_allFV a s)
+| false_prop0 => s
+| multistep_expr a b n => config_allFV a (config_allFV b (nat_allFV n s))
+| multistep'_expr a b n => config_allFV a (config_allFV b s)
+end.
+
+Fixpoint list_prop0_allFV(x:list prop0_expr)(s:S):S :=
+match x with
+| nil => s
+| h::t => prop0_allFV h (list_prop0_allFV t s)
+end.
+
+Definition prop_allFV(x:prop_expr)(s:S):S :=
+let '(H,G):=x in
+list_prop0_allFV H (list_prop0_allFV G s).
+
+End allFV.
+
+Module SimplExpr.
+
+Definition simpl_nat x :=
+  simpls_nat_expr (simpl_nat_expr_by_affine_map x).
+
+Fixpoint simpl_seg(x:seg_expr) :=
+match x with
+| seg_sym a => x
+| seg_concat a b => seg_concat (simpl_seg a) (simpl_seg b)
+| seg_repeat a n => seg_repeat (simpl_seg a) (simpl_nat n)
+| seg_var i => x
+end.
+
+Fixpoint simpl_side(x:side_expr) :=
+match x with
+| side_0inf => x
+| side_var i => x
+| side_concat a b => side_concat (simpl_seg a) (simpl_side b)
+end.
+
+Definition simpl_config(x:config_expr) :=
+let '(l,r,q,d):=x in
+(simpl_side l,simpl_side r,q,d).
+
+Definition simpl_prop0(x:prop0_expr) :=
+match x with
+| nat_eq a b => nat_eq (simpl_nat a) (simpl_nat b)
+| seg_eq a b => seg_eq (simpl_seg a) (simpl_seg b)
+| side_eq a b => side_eq (simpl_side a) (simpl_side b)
+| config_eq a b => config_eq (simpl_config a) (simpl_config b)
+| false_prop0 => false_prop0
+| multistep_expr x0 x1 n => multistep_expr (simpl_config x0) (simpl_config x1) (simpl_nat n)
+| multistep'_expr x0 x1 n => multistep'_expr (simpl_config x0) (simpl_config x1) n
+end.
+
+Definition simpl_prop0_list(x:list prop0_expr) :=
+map simpl_prop0 x.
+
+Definition simpl_prop(x:prop_expr) :=
+let (H,G):=x in
+(simpl_prop0_list H,simpl_prop0_list G).
+
+End SimplExpr.
+
+Module SubstExpr.
+Section subst_expr.
+
+Hypothesis mp: id_t -> forall t:type_t, to_expr_type t.
+Hypothesis mpi: nat_expr.
+
+Fixpoint subst_nat(x:nat_expr) :=
+match x with
+| from_nat n => x
+| nat_add a b => nat_add (subst_nat a) (subst_nat b)
+| nat_mul a b => nat_mul (subst_nat a) (subst_nat b)
+| nat_var i => (mp i nat_t)
+| nat_ivar => mpi
+end.
+
+Fixpoint subst_seg(x:seg_expr) :=
+match x with
+| seg_sym a => x
+| seg_concat a b => seg_concat (subst_seg a) (subst_seg b)
+| seg_repeat a n => seg_repeat (subst_seg a) (subst_nat n)
+| seg_var i => (mp i seg_t)
+end.
+
+Fixpoint subst_side(x:side_expr) :=
+match x with
+| side_0inf => x
+| side_var i => (mp i side_t)
+| side_concat a b => side_concat (subst_seg a) (subst_side b)
+end.
+
+Definition subst_expr(t:type_t)(x:to_expr_type t):to_expr_type t.
+destruct t.
+- apply (subst_nat x).
+- apply (subst_seg x).
+- apply (subst_side x).
+Defined.
+
+Definition subst_config(x:config_expr) :=
+let '(l,r,q,d):=x in
+(subst_side l,subst_side r,q,d).
+
+Definition subst_prop0(x:prop0_expr) :=
+match x with
+| nat_eq a b => nat_eq (subst_nat a) (subst_nat b)
+| seg_eq a b => seg_eq (subst_seg a) (subst_seg b)
+| side_eq a b => side_eq (subst_side a) (subst_side b)
+| config_eq a b => config_eq (subst_config a) (subst_config b)
+| false_prop0 => false_prop0
+| multistep_expr x0 x1 n => multistep_expr (subst_config x0) (subst_config x1) (subst_nat n)
+| multistep'_expr x0 x1 n => multistep'_expr (subst_config x0) (subst_config x1) n
+end.
+
+Definition subst_prop0_list(x:list prop0_expr) :=
+map subst_prop0 x.
+
+Definition subst_prop(x:prop_expr) :=
+let (H,G):=x in
+(subst_prop0_list H,subst_prop0_list G).
+
+End subst_expr.
+End SubstExpr.
+
+
+
+Definition mk_var i t: to_expr_type t :=
+match t with
+| nat_t => nat_var i
+| seg_t => seg_var i
+| side_t => side_var i
+end.
+
+Definition lookup_var t t0 (v:to_expr_type t)(v0:to_expr_type t0):to_expr_type t0.
+  destruct t,t0.
+  all: try (exact v).
+  all: exact v0.
+Defined.
+
+
+Definition subst_vars(mp:PositiveMap.tree expr_expr)(i0:id_t)(t0:type_t):to_expr_type t0 :=
+  match PositiveMap.find i0 mp with
+  | None => mk_var i0 t0
+  | Some (existT _ t v) => lookup_var t t0 v (mk_var i0 t0)
+  end.
+
+Definition subst_identity(i0:id_t)(t0:type_t):to_expr_type t0 :=
+  mk_var i0 t0.
+
+Definition rename_var_by_add(di:id_t)(i0:id_t)(t0:type_t):to_expr_type t0 :=
+  mk_var (i0+di)%positive t0.
+
+Definition rename_var_by_sort(x:prop_expr) :=
+  let (f,p):=prop_allFV x S0 in
+  (SubstExpr.subst_prop (fun i t =>
+    match PositiveMap.find i f with
+    | None => mk_var i t
+    | Some i1 => mk_var i1 t
+    end) nat_ivar x,p).
+
+Module TrySubst.
+Record Config := {
+  enable_subst_exgcd : bool;
+  enable_eq_sym : bool;
+  allowed_lhs_vars : id_t->bool;
+}.
+
+Definition config_normal:= {|
+  enable_subst_exgcd := true;
+  enable_eq_sym := true;
+  allowed_lhs_vars := fun _ => true;
+|}.
+
+Definition config_limited(l r:id_t) := {|
+  enable_subst_exgcd := false;
+  enable_eq_sym := false;
+  allowed_lhs_vars := fun i0 => (l<=?i0)%positive && (i0<=?r)%positive;
+|}.
+
+Section TrySubst_config.
+Hypothesis cfg:Config.
+
+(* lhs vars, rhs vars, fresh var *)
+Definition subst_state:Type :=
+  (PositiveMap.tree expr_expr)*(PositiveMap.tree unit)*id_t.
+
+Definition subst1(l1:id_t)(e:expr_expr)(s:subst_state):subst_state :=
+if negb (cfg.(allowed_lhs_vars) l1) then s else
+let '(sl,sr,p'):=s in
+match PositiveMap.find l1 sl with (* l1 not in sl *)
+| Some _ => s
+| None =>
+  let (r1,_):=(expr_allFV e S0) in
+  if PositiveMap.fold (fun k v s0 =>
+    match PositiveMap.find k sl with
+    | Some _ => true
+    | None => s0
+    end) r1 false
+  then s
+  else (* x in r1 -> x not in dom sl *)
+    let sr':=PositiveMap.fold (fun k v s0 => PositiveMap.add k tt s0) r1 sr in (* sr += r1 *)
+    match PositiveMap.find l1 sr' with
+    | Some _ => s
+    | None => (* l1 not in sr *)
+      let sl' := PositiveMap.add l1 e sl in (* sl += (l1,e) *)
+      (sl',sr,p')
+    end
+end.
+
+Definition fresh_var(s:subst_state):id_t*subst_state :=
+let '(sl,sr,p):=s in
+(p,(sl,sr,Pos.succ p)).
+
+Definition to_affine_1d(x:nat_expr):option (id_t*N*N) :=
+match x with
+| nat_var i => Some (i,1,0)
+| nat_mul (nat_var i) (from_nat k) => Some (i,k,0)
+| nat_add (nat_var i) (from_nat k0) => Some (i,1,k0)
+| nat_add (nat_mul (nat_var i) (from_nat k)) (from_nat k0) => Some (i,k,k0)
+| _ => None
+end%N.
+
+Definition find_subst_exgcd'(x y:id_t)(a b c:N)(s:subst_state):subst_state :=
+  let (x',y') := exgcd a b in
+  if
+    (N.gcd a b =? 1)%N &&
+    negb (a =? 0)%N &&
+    negb (b =? 0)%N &&
+    (a * x' mod b =? 1 mod b)%N &&
+    (b * y' mod a =? 1 mod a)%N
+  then
+    let s:=
+    (if (a =? 1)%N then s else
+    let (i,s):=fresh_var s in
+    subst1 y (make_expr_expr nat_t (nat_add (nat_mul (nat_var i) (from_nat a)) (from_nat ((a-((c*y') mod a)) mod a)))) s) in
+
+    (if (b =? 1)%N then s else
+    let (i,s):=fresh_var s in
+    subst1 x (make_expr_expr nat_t (nat_add (nat_mul (nat_var i) (from_nat b)) (from_nat ((c*x') mod b)))) s)
+  else
+    s.
+
+Definition find_subst_exgcd(a b:nat_expr)(s:subst_state):subst_state :=
+match to_affine_1d a,to_affine_1d b with
+| Some (a0,a1,a2),Some (b0,b1,b2) =>
+  if (a2 =? 0)%N then
+    find_subst_exgcd' a0 b0 a1 b1 b2 s
+  else if (b2 =? 0)%N then
+    find_subst_exgcd' b0 a0 b1 a1 a2 s
+  else
+    s
+| _,_ => s
+end.
+
+
+Definition find_subst(x:prop0_expr)(s:subst_state):subst_state :=
+match x with
+| nat_eq (nat_var i0) b => subst1 i0 (make_expr_expr nat_t b) s
+| nat_eq a b => if cfg.(enable_subst_exgcd) then find_subst_exgcd a b s else s
+| seg_eq (seg_var i0) b => subst1 i0 (make_expr_expr seg_t b) s
+| side_eq (side_var i0) b => subst1 i0 (make_expr_expr side_t b) s
+| _ => s
+end.
+
+Definition simpl_eq(x:prop0_expr):prop0_expr :=
+match x with
+| nat_eq a (nat_var i0) => nat_eq (nat_var i0) a
+| seg_eq a (seg_var i0) => seg_eq (seg_var i0) a
+| side_eq a (side_var i0) => side_eq (side_var i0) a
+| _ => x
+end.
+
+Fixpoint list_find_subst(ls:list prop0_expr)(s:subst_state):subst_state :=
+match ls with
+| nil => s
+| h0::t =>
+  let h:=(if cfg.(enable_eq_sym) then simpl_eq h0 else h0) in
+  list_find_subst t (find_subst h s)
+end.
+
+Definition try_subst(x:prop_expr)(i:id_t) :=
+let (H,G):=x in
+let '(sl,_,p):=list_find_subst H (PositiveMap.empty _,PositiveMap.empty _,i) in
+((SubstExpr.subst_prop (subst_vars sl) nat_ivar x,p),sl).
+
+End TrySubst_config.
+End TrySubst.
+
+
+
+Definition solve_assumptions_iter_limit:nat := 16.
+
+Fixpoint solve_assumptions(n:nat)(cfg:TrySubst.Config)(x:prop_expr)(i:id_t):option (prop_expr*_) :=
+match n with
+| O => None
+| Datatypes.S n0 =>
+  let x0:=x in
+  let x:=prop_solve_eq x in
+  if prop_has_false x then None else
+  let '((x,i),mp0):=TrySubst.try_subst cfg x i in
+  if list_prop0_eqb (fst x) nil then Some (x,mp0::nil) else
+  if prop_eqb x x0 then Some (x,mp0::nil) else (* allow non-empty assumptions *)
+  match solve_assumptions n0 cfg x i with
+  | None => None
+  | Some (x',mp0') => Some (x',mp0::mp0')
+  end
+end.
+
+Definition prop_expr':Type := prop_expr*id_t.
+
+Definition simpl_rule(x:prop_expr):prop_expr' :=
+  let x:=SimplExpr.simpl_prop x in
+  (rename_var_by_sort x).
+
+
+Definition prop_merge(x1 x2:prop_expr)(di:id_t):prop_expr :=
+let (H1,G1):=x1 in
+let (H2,G2):=SubstExpr.subst_prop (rename_var_by_add di) nat_ivar x2 in
+(H1++H2,G1++G2).
+
+Definition prop_multistep'_trans(x:prop_expr): option prop_expr :=
+match x with
+| (H,[multistep'_expr s1 s2 n1;multistep'_expr s3 s4 n2]) => Some ((config_eq s2 s3)::H,[multistep'_expr s1 s4 (n1||n2)])
+| _ => None
+end.
+
+Definition prop_multistep'_apply(x1 x2:prop_expr): option prop_expr :=
+match x1,x2 with
+| ([],[multistep'_expr s1 s2 n1]),([],[multistep'_expr s3 s4 n2]) =>
+  if n1 || negb n2 then
+    Some ([config_eq s1 s3; config_eq s2 s4],[multistep'_expr s3 s4 n2])
+  else None
+| _,_ => None
+end.
+
+Definition follow_rule(w1 w2:prop_expr'):option prop_expr' :=
+let (x1,i1):=w1 in
+let (x2,i2):=w2 in
+let x:=(prop_merge x1 x2 i1) in
+match prop_multistep'_trans x with
+| None => None
+| Some x =>
+  match solve_assumptions solve_assumptions_iter_limit TrySubst.config_normal x (i1+i2+1)%positive with
+  | None => None
+  | Some (x,_) => Some (simpl_rule x)
+  end
+end.
+
+Module FindIH.
+
+Definition oNmin(a b:option N):option N :=
+match a,b with
+| Some a0,Some b0 => Some (N.min a0 b0)
+| Some a0,None => a
+| None,_ => b
+end.
+
+Module Visit1.
+(* guess induction hypothesis *)
+Section visit.
+
+Definition visit_seg(a b ca cb:seg_expr):option (seg_expr*seg_expr*(list prop0_expr)) :=
+if seg_expr_eqb a b then Some (a,a,[]) else
+match a,b,ca,cb with
+| seg_repeat a0 an,seg_repeat b0 bn,seg_repeat ca0 (from_nat can),seg_repeat cb0 (from_nat cbn) =>
+  if seg_expr_eqb a0 b0 && seg_expr_eqb a0 ca0 && seg_expr_eqb a0 cb0 then
+    if (can <=? cbn)%N then (* inc *)
+      let d := (cbn-can)%N in
+      let an' := (nat_add an (nat_mul (nat_ivar) (from_nat d))) in
+      Some (seg_repeat a0 an,seg_repeat a0 an',[nat_eq (nat_add an (from_nat d)) bn]) (* inc *)
+    else (* dec *)
+      let d := (can-cbn)%N in
+      let bn' := (nat_add bn (nat_mul (nat_ivar) (from_nat d))) in
+      Some (seg_repeat b0 bn',seg_repeat b0 bn,[nat_eq (nat_add bn (from_nat d)) an]) (* dec *)
+  else None
+| _,_,_,_ => None
+end.
+
+Fixpoint visit_side(a b ca cb:side_expr):option (side_expr*side_expr*(list prop0_expr)) :=
+match a,b,ca,cb with
+| side_concat a0 a1,side_concat b0 b1,side_concat ca0 ca1,side_concat cb0 cb1 =>
+  match visit_seg a0 b0 ca0 cb0 with
+  | None => None
+  | Some (v0,v0',H0) =>
+    match visit_side a1 b1 ca1 cb1 with
+    | None => None
+    | Some (v1,v1',H1) => Some (side_concat v0 v1,side_concat v0' v1',H0++H1)
+    end
+  end
+| side_var a0,side_var b0,_,_ => if side_expr_eqb a b then Some (a,a,[]) else None
+| side_0inf,side_0inf,side_0inf,side_0inf => Some (a,a,[])
+| _,_,_,_ => None
+end.
+
+Definition visit_config(a b c0 c:config_expr) :=
+let '(l1,r1,s1,sgn1):=a in
+let '(l2,r2,s2,sgn2):=b in
+let '(l30,r30,s30,sgn30):=c0 in
+let '(l3,r3,s3,sgn3):=c in
+if q_eqb s1 s2 && q_eqb s1 s30 && q_eqb s1 s3 && dir_eqb sgn1 sgn2 && dir_eqb sgn1 sgn30 && dir_eqb sgn1 sgn3 then
+  match visit_side l1 l2 l30 l3 with
+  | None => None
+  | Some (l4,l4',Hl) =>
+    match visit_side r1 r2 r30 r3 with
+    | None => None
+    | Some (r4,r4',Hr) => Some ((l4,r4,s1,sgn1),(l4',r4',s1,sgn1),Hl++Hr)
+    end
+  end
+else None.
+
+Definition visit_prop0(a:prop0_expr)(c0 c1:config_expr) :=
+match a with
+| multistep'_expr a0 a1 true =>
+  visit_config a0 a1 c0 c1
+| _ => None
+end.
+End visit.
+End Visit1.
+
+Module Visit2. (* guess the value that decrease to near-zero *)
+Section visit.
+Hypothesis n:N.
+
+Definition visit_seg'(c:seg_expr)(p:id_t) :=
+match c with
+| seg_repeat c0 cn => (seg_repeat c0 (nat_var p),Pos.succ p)
+| _ => (c,p)
+end.
+
+Definition visit_seg(a b ca cb:seg_expr)(p:id_t) :=
+match a,b,ca,cb with
+| seg_repeat a0 an,seg_repeat b0 bn,seg_repeat ca0 (from_nat can),seg_repeat cb0 (from_nat cbn) =>
+  if (can <=? cbn)%N then (* inc *)
+    visit_seg' cb p
+  else (* dec *)
+    let d := (can-cbn)%N in
+    let bn' :=
+    match bn with
+    | from_nat x => x
+    | nat_add _ (from_nat x) => x
+    | _ => N0
+    end in
+    if ((cbn-bn')/d =? n)%N then
+      (seg_repeat b0 (from_nat (((cbn-bn') mod d)+bn')%N),p) (* dec *)
+    else visit_seg' cb p
+| _,_,_,_ => visit_seg' cb p
+end.
+
+Fixpoint visit_side(a b c' c:side_expr)(p:id_t) :=
+match a,b,c',c with
+| side_concat a0 a1,side_concat b0 b1,side_concat c0' c1',side_concat c0 c1 =>
+  let (x0,p):=(visit_seg a0 b0 c0' c0 p) in
+  let (x1,p):=(visit_side a1 b1 c1' c1 p) in
+  (side_concat x0 x1,p)
+| _,_,_,_ => (side_var p,Pos.succ p)
+end.
+
+Definition visit_config(a b c' c:config_expr)(p:id_t) :=
+let '(l1,r1,s1,sgn1):=a in
+let '(l2,r2,s2,sgn2):=b in
+let '(l3',r3',s3',sgn3'):=c' in
+let '(l3,r3,s3,sgn3):=c in
+let (lx,p):=visit_side l1 l2 l3' l3 p in
+let (rx,p):=visit_side r1 r2 r3' r3 p in
+((lx,rx,s2,sgn2),p).
+
+Definition visit_config'(c:config_expr)(p:id_t) :=
+let '(l3,r3,s3,sgn3):=c in
+let (lx,p):=(side_var p,Pos.succ p) in
+let (rx,p):=(side_var p,Pos.succ p) in
+((lx,rx,s3,sgn3),p).
+
+End visit.
+End Visit2.
+
+Module Visit3.
+(* guess n *)
+
+Definition visit_seg(a b ca cb:seg_expr):option N :=
+match a,b,ca,cb with
+| seg_repeat a0 an,seg_repeat b0 bn,seg_repeat ca0 (from_nat can),seg_repeat cb0 (from_nat cbn) =>
+  if (can <=? cbn)%N then (* inc *)
+    None
+  else (* dec *)
+    let d := (can-cbn)%N in
+    let bn' :=
+    match bn with
+    | from_nat x => x
+    | nat_add _ (from_nat x) => x
+    | _ => N0
+    end in
+    Some (1+(cbn-bn')/d)%N (* dec *)
+| _,_,_,_ => None
+end.
+
+Fixpoint visit_side(a b ca cb:side_expr):option N :=
+match a,b,ca,cb with
+| side_concat a0 a1,side_concat b0 b1,side_concat ca0 ca1,side_concat cb0 cb1 =>
+  oNmin (visit_seg a0 b0 ca0 cb0) (visit_side a1 b1 ca1 cb1)
+| _,_,_,_ => None
+end.
+
+Definition visit_config(a b c0 c:config_expr) :=
+let '(l1,r1,s1,sgn1):=a in
+let '(l2,r2,s2,sgn2):=b in
+let '(l30,r30,s30,sgn30):=c0 in
+let '(l3,r3,s3,sgn3):=c in
+oNmin (visit_side l1 l2 l30 l3) (visit_side r1 r2 r30 r3).
+
+End Visit3.
+
+
+Definition find_IH(x:prop_expr)(i:id_t)(x0' x0:prop_expr):option (prop_expr'*(prop_expr')*_*option N) :=
+match x,x0',x0 with
+| (Hx,[a]),([],[multistep'_expr _ c' _]),([],[multistep'_expr _ c _]) =>
+  match Visit1.visit_prop0 a c' c with
+  | None => None
+  | Some (a,b,H) =>
+    match solve_assumptions solve_assumptions_iter_limit TrySubst.config_normal (H++Hx,[multistep'_expr a b false]) i with
+    | Some (Hx',[multistep'_expr a b false],mp) =>
+      let n := Visit3.visit_config a b c' c in
+      let (b',p) :=
+      match n with
+      | None => Visit2.visit_config' c 1%positive
+      | Some n => Visit2.visit_config n a b c' c 1%positive
+      end in
+      let w0 := (simpl_rule (Hx',[multistep'_expr a b false])) in
+      let w1 := ([],[multistep'_expr b' b' false],p) in
+      match n with
+      | None =>
+        match follow_rule ([],[multistep'_expr c' c' false],1%positive) w0 with
+        | Some w0' => Some (simpl_rule (fst w0'),w1,mp,n)
+        | None => None
+        end
+      | Some _ => Some (w0,w1,mp,n)
+      end
+    | _ => None
+    end
+  end
+| _,_,_ => None
+end.
+
+End FindIH.
+
+
+
+
+Section tm_ctx.
+Hypothesis tm:TM.
+
+Section subst_var.
+Hypothesis mp:id_t->forall t:type_t, to_type t.
+Hypothesis mpi:N.
+
+Fixpoint to_nat(x:nat_expr) :=
+(match x with
+| from_nat n => n
+| nat_add a b => (to_nat a) + (to_nat b)
+| nat_mul a b => (to_nat a) * (to_nat b)
+| nat_var i => (mp i nat_t)
+| nat_ivar => mpi
+end)%N.
+
+Fixpoint to_seg(x:seg_expr):list Sym :=
+match x with
+| seg_sym a => [a]
+| seg_concat a b => (to_seg a) ++ (to_seg b)
+| seg_repeat a n => (to_seg a) ^^ (N.to_nat (to_nat n))
+| seg_var i => (mp i seg_t)
+end.
+
+Fixpoint to_side(x:side_expr):side :=
+match x with
+| side_0inf => const s0
+| side_var i => (mp i side_t)
+| side_concat a b => to_seg a *> to_side b
+end.
+
+
+Definition to_expr t1 (e1:to_expr_type t1): to_type t1.
+destruct t1; cbn in e1; cbn.
+- apply (to_nat e1).
+- apply (to_seg e1).
+- apply (to_side e1).
+Defined.
+
+Definition to_config(x:config_expr) :=
+let '(l,r,q,d):=x in
+match d with
+| L => (to_side r) <{{q}} (to_side l)
+| R => (to_side l) {{q}}> (to_side r)
+end.
+
+Definition to_prop0(x:prop0_expr):Prop :=
+match x with
+| nat_eq a b => to_nat a = to_nat b
+| seg_eq a b => to_seg a = to_seg b
+| side_eq a b => to_side a = to_side b
+| config_eq a b => to_config a = to_config b
+| false_prop0 => False
+| multistep_expr x0 x1 n => (to_config x0) -[tm]->> (N.to_nat (to_nat n)) / (to_config x1)
+| multistep'_expr x0 x1 n => multistep' tm n (to_config x0) (to_config x1)
+end.
+
+Definition to_prop0_list(x:list prop0_expr):Prop :=
+Forall to_prop0 x.
+
+Definition to_prop(x:prop_expr):Prop :=
+let (H,G):=x in
+to_prop0_list H ->
+to_prop0_list G.
+
+
+Definition affine_map_to_Z(f:affine_map):Z :=
+let (v1,v2):=from_affine_map f in
+(Z.of_N (to_nat v1))-(Z.of_N (to_nat v2)).
+
+
+Lemma affine_map_to_Z_cons x0 y0 f:
+  (affine_map_to_Z ((x0,y0)::f) = (Z.of_N (to_nat x0))*y0 + (affine_map_to_Z f))%Z.
+Proof.
+  unfold affine_map_to_Z.
+  cbn.
+  destruct (from_affine_map f) as [v1 v2].
+  destruct y0 as [|y0|y0]; cbn; lia.
+Qed.
+
+Lemma affine_map_upd'_spec f x u:
+  let (f',t) := affine_map_upd' f x u in
+  if t then (affine_map_to_Z f') = ((affine_map_to_Z f) + (Z.of_N (to_nat x)) * u)%Z
+  else (affine_map_to_Z f') = (affine_map_to_Z f).
+Proof.
+  induction f as [|[x0 y0] f].
+  1: reflexivity.
+  cbn.
+  destruct (affine_map_upd' f x u) as [f' t].
+  destruct (nat_expr_eqb_spec x0 x).
+  - subst.
+    repeat rewrite affine_map_to_Z_cons.
+    lia.
+  - destruct t.
+    + repeat rewrite affine_map_to_Z_cons.
+      lia.
+    + repeat rewrite affine_map_to_Z_cons.
+      lia.
+Qed.
+
+Lemma affine_map_upd_spec f x u:
+  affine_map_to_Z (affine_map_upd f x u) = ((affine_map_to_Z f) + (Z.of_N (to_nat x)) * u)%Z.
+Proof.
+  unfold affine_map_upd.
+  pose proof (affine_map_upd'_spec f x u) as H.
+  destruct (affine_map_upd' f x u) as [f' [|]].
+  - apply H.
+  - rewrite affine_map_to_Z_cons.
+    lia.
+Qed.
+
+Lemma add_to_affine_map_spec a u f:
+  affine_map_to_Z (add_to_affine_map a u f) =
+  ((affine_map_to_Z f)+(Z.of_N (to_nat a))*u)%Z.
+Proof.
+  gen u f.
+  induction a; intros; cbn.
+  - rewrite affine_map_upd_spec.
+    cbn[to_nat]. lia.
+  - rewrite IHa2,IHa1.
+    lia.
+  - destruct a2.
+    1: cbn; rewrite IHa1; lia.
+    all:
+      rewrite affine_map_upd_spec;
+      reflexivity.
+  - rewrite affine_map_upd_spec;
+    reflexivity.
+  - rewrite affine_map_upd_spec.
+    reflexivity.
+Qed.
+
+Lemma affine_map_div_spec f g:
+  g<>Z0 ->
+  affine_map_divide f g ->
+  (let (f0,m0) := (affine_map_div f g) in
+  (affine_map_to_Z f0)*g+m0 = affine_map_to_Z f)%Z.
+Proof.
+  intro Hg.
+  induction f as [|[x0 y0] f]; intros H; cbn.
+  1: reflexivity.
+  cbn in H.
+  destruct (affine_map_div f g) as [f0 m0] eqn:E.
+  repeat rewrite affine_map_to_Z_cons.
+  destruct (nat_expr_eqb_spec x0 (from_nat 1)).
+  + rewrite <-IHf. 2: tauto.
+    rewrite e. change (Z.of_N (to_nat (from_nat 1))) with (1%Z).
+    lia.
+  + destruct H as [[y1 Ha] Hb].
+    subst y0.
+    rewrite Z.div_mul; auto. lia.
+Qed.
+
+Lemma from_affine_map_spec f:
+  let (v1,v2):=from_affine_map f in
+  (affine_map_to_Z f = Z.of_N (to_nat v1) - Z.of_N (to_nat v2))%Z.
+Proof.
+  induction f as [|[x0 y0] f].
+  1: cbn; lia.
+  cbn.
+  rewrite affine_map_to_Z_cons.
+  destruct (from_affine_map f) as [v1 v2].
+  destruct y0 as [|y0|y0]; cbn; lia.
+Qed.
+
+Lemma from_affine_map_spec' f:
+  let (v1,v2):=from_affine_map f in
+  affine_map_to_Z f = Z0 <->
+  to_nat v1 = to_nat v2.
+Proof.
+  pose proof (from_affine_map_spec f) as H.
+  destruct (from_affine_map f) as [v1 v2].
+  lia.
+Qed.
+
+
+Lemma simpl_nat_expr_spec x:
+  to_nat (simpl_nat_expr x) = to_nat x.
+Proof.
+  destruct x.
+  all: try reflexivity.
+  - destruct x1.
+    all: try reflexivity.
+    + destruct n.
+      * reflexivity.
+      * cbn[simpl_nat_expr]. cbn[to_nat]. lia.
+    + destruct x1_2.
+      all: try reflexivity.
+      cbn. lia.
+  - destruct x1,x2; cbn.
+    all: try reflexivity.
+    all: destruct n as [|[n|n|]];
+    try reflexivity.
+    all: try destruct n0 as [|[n0|n0|]];
+    try reflexivity.
+    all: cbn[to_nat]; lia.
+Qed.
+
+Lemma simpls_nat_expr_spec x:
+  to_nat (simpls_nat_expr x) = to_nat x.
+Proof.
+  induction x.
+  all: try reflexivity.
+  - cbn[simpls_nat_expr].
+    repeat rewrite simpl_nat_expr_spec.
+    cbn.
+    congruence.
+  - cbn[simpls_nat_expr].
+    repeat rewrite simpl_nat_expr_spec.
+    cbn.
+    congruence.
+Qed.
+
+Lemma simpl_nat_expr_by_affine_map_spec x:
+  to_nat (simpl_nat_expr_by_affine_map x) = to_nat x.
+Proof.
+  unfold simpl_nat_expr_by_affine_map.
+  pose proof (from_affine_map_spec (add_to_affine_map x 1 [])) as H.
+  destruct (from_affine_map (add_to_affine_map x 1 [])) as [v1 v2].
+  destruct (nat_expr_eqb_spec v2 (from_nat 0)).
+  2: reflexivity.
+  subst v2.
+  rewrite add_to_affine_map_spec in H.
+  cbn in H.
+  lia.
+Qed.
+
+Lemma list_prop0_from_affine_map_spec f:
+  to_prop0_list (list_prop0_from_affine_map f) ->
+  affine_map_to_Z f = Z0.
+Proof.
+  unfold list_prop0_from_affine_map.
+  intro H.
+  pose proof (from_affine_map_spec f) as H0.
+  remember (from_affine_map f) as v.
+  assert (let (v1,v2):=v in to_nat v1 = to_nat v2) as H'. {
+    destruct v as [v1 v2].
+    destruct (nat_expr_eqb_spec v1 v2).
+    - congruence.
+    - unfold to_prop0_list in H.
+      rewrite Forall_cons_iff in H.
+      cbn in H.
+      repeat rewrite simpls_nat_expr_spec in H.
+      tauto.
+  }
+  destruct v as [v1 v2].
+  lia.
+Qed.
+
+Lemma from_affine_map_simpl_div_spec f:
+  to_prop0_list (from_affine_map_simpl_div f) ->
+  affine_map_to_Z f = Z0.
+Proof.
+  unfold from_affine_map_simpl_div.
+  intro H.
+  destruct (Z.ltb_spec 1 (affine_map_gcd f)).
+  2: apply list_prop0_from_affine_map_spec,H.
+  pose proof (affine_map_gcd_spec f).
+  remember (affine_map_gcd f) as g.
+  pose proof (affine_map_div_spec f g).
+  destruct (affine_map_div f g) as [f0 g0].
+  destruct (Z.eqb_spec g0 0).
+  - rewrite <-H2.
+    + rewrite list_prop0_from_affine_map_spec; auto.
+    + lia.
+    + tauto.
+  - destruct (Z.eqb (g0 mod g) 0).
+    1: apply list_prop0_from_affine_map_spec,H.
+    unfold to_prop0_list in H.
+    rewrite Forall_cons_iff in H.
+    cbn in H. tauto.
+Qed.
+
+Lemma solve_nat_eq_spec a b:
+  to_prop0_list (solve_nat_eq a b) ->
+  to_prop0 (nat_eq a b).
+Proof.
+  cbn.
+  intro E.
+  unfold solve_nat_eq in E.
+  pose proof (from_affine_map_simpl_div_spec _ E) as H'.
+  repeat rewrite add_to_affine_map_spec in H'.
+  cbn in H'. lia.
+Qed.
+
+Lemma solve_seg_eq_spec a b:
+  to_prop0_list (solve_seg_eq a b) ->
+  to_prop0 (seg_eq a b).
+Proof.
+  cbn.
+  gen b.
+  induction a; intros b E; destruct b; unfold to_prop0_list in E; cbn; cbn in E.
+  all: repeat (rewrite Forall_cons_iff in E; cbn in E).
+  all: try tauto.
+  - destruct (sym_eqb_spec a a0); try congruence.
+    repeat rewrite Forall_cons_iff in E.
+    cbn in E.
+    tauto.
+  - rewrite Forall_app in E.
+    rewrite (IHa1 b1). 2: tauto.
+    rewrite (IHa2 b2). 2: tauto.
+    reflexivity.
+  - rewrite Forall_app in E.
+    rewrite (IHa b). 2: tauto.
+    rewrite (solve_nat_eq_spec n n0). 2: tauto.
+    reflexivity.
+  - destruct (Pos.eqb_spec i i0).
+    + congruence.
+    + rewrite Forall_cons_iff in E.
+      cbn in E.
+      tauto.
+Qed.
+
+Lemma solve_side_eq_spec a b:
+  to_prop0_list (solve_side_eq a b) ->
+  to_prop0 (side_eq a b).
+Proof.
+  gen b.
+  induction a; intros b E; destruct b; unfold to_prop0_list in E; cbn; cbn in E.
+  all: repeat (rewrite Forall_cons_iff in E; cbn in E).
+  all: try tauto.
+  - destruct (Pos.eqb_spec i i0).
+    + congruence.
+    + rewrite Forall_cons_iff in E.
+      cbn in E.
+      tauto.
+  - rewrite Forall_app in E.
+    rewrite (IHa b). 2: tauto.
+    rewrite (solve_seg_eq_spec a a1). 2: tauto.
+    reflexivity.
+Qed.
+
+Lemma solve_config_eq_spec a b:
+  to_prop0_list (solve_config_eq a b) ->
+  to_prop0 (config_eq a b).
+Proof.
+  destruct a as [[[l1 r1] s1] d1].
+  destruct b as [[[l2 r2] s2] d2].
+  cbn.
+  destruct (q_eqb_spec s1 s2).
+  - destruct (dir_eqb_spec d1 d2).
+    + subst.
+      unfold to_prop0_list.
+      rewrite Forall_app.
+      intros [Ha Hb].
+      pose proof (solve_side_eq_spec l1 l2 Ha) as H1.
+      pose proof (solve_side_eq_spec r1 r2 Hb) as H2.
+      cbn in H1,H2.
+      rewrite H1,H2.
+      congruence.
+    + unfold to_prop0_list; cbn; rewrite Forall_cons_iff; cbn; tauto.
+  - unfold to_prop0_list; cbn; rewrite Forall_cons_iff; cbn; tauto.
+Qed.
+
+Lemma solve_eq_spec x:
+  to_prop0_list (solve_eq x) ->
+  to_prop0 x.
+Proof.
+  destruct x; cbn.
+  - apply solve_nat_eq_spec.
+  - apply solve_seg_eq_spec.
+  - apply solve_side_eq_spec.
+  - apply solve_config_eq_spec.
+  - unfold to_prop0_list.
+    rewrite Forall_cons_iff; cbn; tauto.
+  - unfold to_prop0_list.
+    rewrite Forall_cons_iff; cbn; tauto.
+  - unfold to_prop0_list.
+    rewrite Forall_cons_iff; cbn; tauto.
+Qed.
+
+
+Lemma solve_eqs_spec x:
+  to_prop0_list (solve_eqs x) ->
+  to_prop0_list x.
+Proof.
+  induction x; cbn.
+  1: tauto.
+  unfold to_prop0_list.
+  rewrite Forall_app.
+  rewrite Forall_cons_iff.
+  pose proof (solve_eq_spec a).
+  tauto.
+Qed.
+
+Lemma has_false_spec x:
+  has_false x = true ->
+  to_prop0_list x ->
+  False.
+Proof.
+  induction x.
+  - cbn. congruence.
+  - cbn.
+    destruct a; cbn.
+    all: unfold to_prop0_list.
+    all: unfold to_prop0_list in IHx.
+    all: rewrite Forall_cons_iff.
+    all: tauto.
+Qed.
+
+
+
+
+
+Section ExprEq_spec.
+Import ExprEq.
+
+Lemma ExprEq_nat_spec a b:
+  nat_expr_eqb a b = true ->
+  to_nat a = to_nat b.
+Proof.
+  unfold nat_expr_eqb.
+  pose proof (solve_nat_eq_spec a b).
+  destruct (solve_nat_eq a b).
+  2: congruence.
+  intros _.
+  apply H.
+  constructor.
+Qed.
+
+Lemma ExprEq_seg_spec a b:
+  seg_expr_eqb a b = true ->
+  to_seg a = to_seg b.
+Proof.
+  gen b.
+  induction a; intros b; destruct b; cbn; try congruence;
+  repeat rewrite and_true_iff.
+  - destruct (sym_eqb_spec a a0); congruence.
+  - intros [H1 H2].
+    erewrite IHa1; eauto.
+    erewrite IHa2; eauto.
+  - intros [H1 H2].
+    erewrite IHa; eauto.
+    erewrite ExprEq_nat_spec; eauto.
+  - destruct (Pos.eqb_spec i i0); congruence.
+Qed.
+
+Lemma ExprEq_side_spec a b:
+  side_expr_eqb a b = true ->
+  to_side a = to_side b.
+Proof.
+  gen b.
+  induction a; intros b; destruct b; cbn; try congruence;
+  repeat rewrite and_true_iff.
+  - destruct (Pos.eqb_spec i i0); congruence.
+  - intros [H1 H2].
+    erewrite IHa; eauto.
+    erewrite ExprEq_seg_spec; eauto.
+Qed.
+
+Lemma ExprEq_config_spec a b:
+  config_expr_eqb a b = true ->
+  to_config a = to_config b.
+Proof.
+  destruct a as [[[l1 r1] s1] sgn1].
+  destruct b as [[[l2 r2] s2] sgn2].
+  cbn.
+  repeat rewrite and_true_iff.
+  intros [[[H0 H1] H2] H3].
+  rewrite (ExprEq_side_spec l1 l2); auto.
+  rewrite (ExprEq_side_spec r1 r2); auto.
+  destruct (q_eqb_spec s1 s2); try congruence.
+  destruct (dir_eqb_spec sgn1 sgn2); try congruence.
+  subst. reflexivity.
+Qed.
+
+Lemma ExprEq_prop0_spec a b:
+  prop0_eqb a b = true ->
+  to_prop0 a = to_prop0 b.
+Proof.
+  destruct a,b; cbn;
+  repeat rewrite and_true_iff;
+  try congruence.
+  - intros [H1 H2].
+    rewrite (ExprEq_nat_spec a a0); auto.
+    rewrite (ExprEq_nat_spec b0 b); auto.
+  - intros [H1 H2].
+    rewrite (ExprEq_seg_spec a a0); auto.
+    rewrite (ExprEq_seg_spec b0 b); auto.
+  - intros [H1 H2].
+    rewrite (ExprEq_side_spec a a0); auto.
+    rewrite (ExprEq_side_spec b0 b); auto.
+  - intros [H1 H2].
+    rewrite (ExprEq_config_spec a a0); auto.
+    rewrite (ExprEq_config_spec b0 b); auto.
+  - intros [[H1 H2] H3].
+    rewrite (ExprEq_config_spec a a0); auto.
+    rewrite (ExprEq_config_spec b0 b); auto.
+    rewrite (ExprEq_nat_spec n n0); auto.
+  - intros [[H1 H2] H3].
+    rewrite (ExprEq_config_spec a a0); auto.
+    rewrite (ExprEq_config_spec b0 b); auto.
+    destruct (Bool.eqb_spec n n0); congruence.
+Qed.
+
+Lemma ExprEq_list_prop0_spec a b:
+  list_prop0_eqb a b = true ->
+  to_prop0_list a <-> to_prop0_list b.
+Proof.
+  unfold to_prop0_list.
+  gen b.
+  induction a as [|a0 a]; intros [|b0 b]; cbn; try congruence;
+  repeat rewrite and_true_iff.
+  1: tauto.
+  intros [H1 H2].
+  repeat rewrite Forall_cons_iff.
+  rewrite (ExprEq_prop0_spec a0 b0); try tauto.
+  rewrite (IHa b); tauto.
+Qed.
+
+Lemma ExprEq_prop_spec a b:
+  prop_eqb a b = true ->
+  to_prop a <-> to_prop b.
+Proof.
+  destruct a as [a0 a1].
+  destruct b as [b0 b1].
+  cbn; try congruence;
+  repeat rewrite and_true_iff.
+  intros [H1 H2].
+  rewrite (ExprEq_list_prop0_spec _ _ H1).
+  rewrite (ExprEq_list_prop0_spec _ _ H2).
+  tauto.
+Qed.
+
+End ExprEq_spec.
+
+
+Section simpl_spec.
+Import SimplExpr.
+Lemma nat_simpl_spec x:
+  to_nat (simpl_nat x) = to_nat x.
+Proof.
+  unfold simpl_nat.
+  rewrite simpls_nat_expr_spec.
+  apply simpl_nat_expr_by_affine_map_spec.
+Qed.
+
+Lemma seg_simpl_spec x:
+  to_seg (simpl_seg x) = to_seg x.
+Proof.
+  induction x; cbn.
+  all: try congruence.
+  rewrite (nat_simpl_spec n).
+  congruence.
+Qed.
+
+Lemma side_simpl_spec x:
+  to_side (simpl_side x) = to_side x.
+Proof.
+  induction x; cbn.
+  all: try congruence.
+  rewrite seg_simpl_spec.
+  congruence.
+Qed.
+
+Lemma config_simpl_spec x:
+  to_config (simpl_config x) = to_config x.
+Proof.
+  destruct x as [[[l r] s] sgn]; cbn.
+  destruct sgn;
+  repeat rewrite side_simpl_spec;
+  congruence.
+Qed.
+
+Lemma prop0_simpl_spec x:
+  to_prop0 (simpl_prop0 x) = to_prop0 x.
+Proof.
+  destruct x; cbn.
+  all: repeat rewrite nat_simpl_spec.
+  all: repeat rewrite seg_simpl_spec.
+  all: repeat rewrite side_simpl_spec.
+  all: repeat rewrite config_simpl_spec.
+  all: try congruence.
+Qed.
+
+Lemma list_prop0_simpl_spec x:
+  to_prop0_list (simpl_prop0_list x) <-> to_prop0_list x.
+Proof.
+  unfold to_prop0_list.
+  induction x; cbn.
+  - repeat rewrite Forall_nil_iff; tauto.
+  - repeat rewrite Forall_cons_iff.
+    rewrite prop0_simpl_spec; tauto.
+Qed.
+
+Lemma prop_simpl_spec x:
+  to_prop (simpl_prop x) <-> to_prop x.
+Proof.
+  destruct x as [x0 x1]; cbn.
+  repeat rewrite list_prop0_simpl_spec.
+  tauto.
+Qed.
+
+End simpl_spec.
+
+End subst_var.
+
+
+
+Section subst_spec.
+Import SubstExpr.
+Hypothesis mp':id_t->forall t, to_type t.
+Hypothesis mpi':N.
+Hypothesis mp0:id_t->forall t, to_expr_type t.
+Hypothesis mpi0:nat_expr.
+Definition mp(i:id_t) t: to_type t := (to_expr mp' mpi' t (mp0 i t)).
+Definition mpi:N := to_expr mp' mpi' nat_t mpi0.
+
+Lemma nat_subst_spec x:
+  to_nat mp' mpi' (subst_nat mp0 mpi0 x) = to_nat mp mpi x.
+Proof.
+  induction x.
+  - reflexivity.
+  - cbn.
+    rewrite IHx1,IHx2.
+    reflexivity.
+  - cbn.
+    rewrite IHx1,IHx2.
+    reflexivity.
+  - reflexivity.
+  - reflexivity.
+Qed.
+
+Lemma seg_subst_spec x:
+  to_seg mp' mpi' (subst_seg mp0 mpi0 x) = to_seg mp mpi x.
+Proof.
+  induction x.
+  - reflexivity.
+  - cbn.
+    rewrite IHx1,IHx2.
+    reflexivity.
+  - cbn.
+    rewrite IHx,nat_subst_spec.
+    reflexivity.
+  - reflexivity.
+Qed.
+
+Lemma side_subst_spec x:
+  to_side mp' mpi' (subst_side mp0 mpi0 x) = to_side mp mpi x.
+Proof.
+  induction x.
+  - reflexivity.
+  - reflexivity.
+  - cbn.
+    rewrite IHx,seg_subst_spec.
+    reflexivity.
+Qed.
+
+Lemma config_subst_spec x:
+  to_config mp' mpi' (subst_config mp0 mpi0 x) = to_config mp mpi x.
+Proof.
+  destruct x as [[[l r] s] sgn].
+  cbn.
+  destruct sgn;
+  repeat rewrite side_subst_spec;
+  reflexivity.
+Qed.
+
+Lemma prop0_subst_spec x:
+  to_prop0 mp' mpi' (subst_prop0 mp0 mpi0 x) = to_prop0 mp mpi x.
+Proof.
+  destruct x; cbn.
+  - repeat rewrite nat_subst_spec.
+    reflexivity.
+  - repeat rewrite seg_subst_spec.
+    reflexivity.
+  - repeat rewrite side_subst_spec.
+    reflexivity.
+  - repeat rewrite config_subst_spec.
+    reflexivity.
+  - reflexivity.
+  - repeat rewrite config_subst_spec.
+    repeat rewrite nat_subst_spec.
+    reflexivity.
+  - repeat rewrite config_subst_spec.
+    reflexivity.
+Qed.
+
+Lemma prop0_list_subst_spec x:
+  to_prop0_list mp' mpi' (subst_prop0_list mp0 mpi0 x) <-> to_prop0_list mp mpi x.
+Proof.
+  unfold to_prop0_list.
+  induction x; cbn.
+  - repeat rewrite Forall_nil_iff; tauto.
+  - repeat rewrite Forall_cons_iff.
+    rewrite prop0_subst_spec.
+    tauto.
+Qed.
+
+Lemma prop_subst_spec x:
+  to_prop mp' mpi' (subst_prop mp0 mpi0 x) <-> to_prop mp mpi x.
+Proof.
+  destruct x; cbn.
+  repeat rewrite prop0_list_subst_spec.
+  tauto.
+Qed.
+
+End subst_spec.
+
+
+
+
+
+
+Lemma multistep'_trans n1 n2 s1 s2 s3:
+  multistep' tm n1 s1 s2 ->
+  multistep' tm n2 s2 s3 ->
+  multistep' tm (n1||n2) s1 s3.
+Proof.
+  unfold multistep'.
+  destruct n1,n2; cbn.
+  - apply progress_trans.
+  - apply progress_evstep_trans.
+  - apply evstep_progress_trans.
+  - apply evstep_trans.
+Qed.
+
+
+
+
+
+
+
+
+
+
+Definition match_prop(x1 x2:prop_expr):option prop_expr :=
+match x1,x2 with
+| ([],[multistep'_expr s1 s2 n1]),([],[multistep'_expr s1' s2' n1']) =>
+  Some ([config_eq s1 s1';config_eq s2 s2'],[])
+| _,_ => None
+end.
+
+(*
+  substitute variables in w1,
+  then prove w1 <-> w2 by ExprEq.prop_eqb
+
+  (forall x, w1(x)) ->
+  (forall x, w1(f(x)) <-> w2(x)) ->
+  (forall x, w2(x))
+*)
+Definition subst_for_apply(w1 w2:prop_expr'):option _:=
+let (x1,i1):=w1 in
+let (x2,i2):=w2 in
+let x1' := SubstExpr.subst_prop (rename_var_by_add i2) nat_ivar x1 in
+match match_prop x1' x2 with
+| None => None
+| Some x3 =>
+  match solve_assumptions solve_assumptions_iter_limit (TrySubst.config_limited i2 (i1+i2)%positive) x3 (i1+i2+1)%positive with
+  | None => None
+  | Some (x,mp0s) =>
+    let mp0 := List.fold_left
+      (fun mp0s mp0 => PositiveMap.fold (fun k v f => PositiveMap.add (k-i2)%positive v f) mp0 mp0s)
+      mp0s (PositiveMap.empty _) in
+      Some mp0
+  end
+end.
+
+Definition solve_apply(w1 w2:prop_expr'):bool :=
+match subst_for_apply w1 w2 with
+| None => false
+| Some mp0 =>
+  let x1' := (SubstExpr.subst_prop (subst_vars mp0) nat_ivar (fst w1)) in
+  ExprEq.prop_eqb x1' (fst w2)
+end.
+
+
+(*
+  prove w by induction,
+  prove base case by wO,
+  prove induction step by "follow wS; follow IH; finish"
+*)
+Definition solve_ind(wO wS w:prop_expr'):bool :=
+match follow_rule w wS with
+| None => false
+| Some w' =>
+  solve_apply wO ((SubstExpr.subst_prop subst_identity (from_nat 0) (fst w)),(snd w)) &&
+  solve_apply w' ((SubstExpr.subst_prop subst_identity (nat_add nat_ivar (from_nat 1)) (fst w)),(snd w))
+end.
+
+Definition step0_refl s sgn:prop_expr' :=
+  let l:=side_var 1%positive in
+  let r:=side_var 2%positive in
+  (([],[multistep'_expr (l,r,s,sgn) (l,r,s,sgn) false]),
+  3%positive).
+
+Definition get_config_r(x:prop_expr') :=
+let '((H,G),i):=x in
+match G with
+| (multistep'_expr a b n)::_ => Some b
+| _ => None
+end.
+
+Definition find_step0_refl(x:prop_expr'):option prop_expr' :=
+match get_config_r x with
+| Some (_,_,s,sgn) => Some (step0_refl s sgn)
+| None => None
+end.
+
+Definition step1_to_step0(x:prop_expr'):prop_expr' :=
+match x with
+| (H,(multistep'_expr a b true)::G,i) =>
+  (H,(multistep'_expr a b false)::G,i)
+| _ => x
+end.
+
+Definition remove_ivar(x:prop_expr'):prop_expr' :=
+let (x,i):=x in
+let x:=SubstExpr.subst_prop subst_identity (nat_var i) x in
+simpl_rule x.
+
+Definition specialize_ivar(x:prop_expr')(n:N):prop_expr' :=
+let (x,i):=x in
+let x:=SubstExpr.subst_prop subst_identity (from_nat n) x in
+simpl_rule x.
+
+Fixpoint subst_list_map(mp:list (PositiveMap.tree expr_expr))(i:id_t)(t:type_t):to_expr_type t :=
+match mp with
+| nil => mk_var i t
+| mp0::mp =>
+  SubstExpr.subst_expr (subst_list_map mp) nat_ivar t (subst_vars mp0 i t)
+end.
+
+
+Definition subst_ind_S(w:prop_expr') (mp:list (PositiveMap.tree expr_expr)):prop_expr' :=
+  let w1 := step1_to_step0 w in
+  (SubstExpr.subst_prop (subst_list_map mp) nat_ivar (fst w1),snd w1).
+
+(*
+  find accelerate rule w1^n, that can be used after w0
+*)
+Definition try_ind(w1 w0' w0:prop_expr'):option (prop_expr'*prop_expr') :=
+let (x1,i1):=w1 in
+match FindIH.find_IH x1 i1 (fst w0') (fst w0) with
+| Some (w2,x3,mp,n) =>
+  match (find_step0_refl w1) with
+  | None => None
+  | Some w10 =>
+    let w1' := subst_ind_S w1 mp in
+    if solve_ind w10 w1' w2 then
+      match n with
+      | Some n =>
+        if solve_apply w10 x3 then
+          match follow_rule w2 x3 with
+          | None => None
+          | Some w2 =>
+            match follow_rule w0' (specialize_ivar w2 n) with
+            | None => None
+            | Some w0 => Some (remove_ivar w2,w0)
+            end
+          end
+        else None
+      | None =>
+        match follow_rule w0' (remove_ivar w2) with
+        | None => None
+        | Some w0 => Some (remove_ivar w2,w0)
+        end
+      end
+    else None
+  end
+| _ => None
+end.
+
+Definition multistep'_for_ind(w1:prop_expr'):prop_expr' :=
+match w1 with
+| ((H,multistep'_expr a b true::G),i) => ((H,multistep'_expr a b false::G),i)
+| _ => w1
+end.
+
+
+Section ivar.
+Hypothesis mpi:N.
+Definition to_prop'' x :=
+  forall mp, to_prop mp mpi x.
+
+Opaque solve_assumptions_iter_limit.
+
+Lemma subst_spec x mp0:
+  to_prop'' x ->
+  to_prop'' (SubstExpr.subst_prop mp0 nat_ivar x).
+Proof.
+  intros H mp'.
+  rewrite prop_subst_spec.
+  apply H.
+Qed.
+
+Lemma prop_merge_spec x1 x2 di:
+  to_prop'' x1 ->
+  to_prop'' x2 ->
+  to_prop'' (prop_merge x1 x2 di).
+Proof.
+  pose proof (subst_spec x2) as H.
+  gen H.
+  unfold to_prop''.
+  unfold prop_merge.
+  destruct x1 as [H1 G1].
+  destruct x2 as [H2 G2].
+  cbn.
+  unfold to_prop0_list.
+  intros H Hx1 Hx2 mp.
+  repeat rewrite Forall_app.
+  intros.
+  split.
+  - apply Hx1; tauto.
+  - apply H; tauto.
+Qed.
+
+Lemma prop_multistep'_trans_spec x:
+match prop_multistep'_trans x with
+| None => True
+| Some x' => to_prop'' x -> to_prop'' x'
+end.
+Proof.
+  destruct x as [H' G].
+  destruct G as [|G0 G]; cbn; trivial.
+  destruct G0; cbn; trivial.
+  destruct G as [|G0 G]; cbn; trivial.
+  destruct G0; cbn; trivial.
+  destruct G as [|G0 G]; cbn; trivial.
+  unfold to_prop''.
+  cbn.
+  unfold to_prop0_list.
+  intros H mp.
+  specialize (H mp).
+  gen H.
+  repeat rewrite Forall_cons_iff.
+  repeat rewrite Forall_nil_iff.
+  cbn.
+  intros H [H0 H1].
+  rewrite H0 in H.
+  split; trivial.
+  destruct (H H1) as [Ha [Hb _]].
+  eapply multistep'_trans; eauto.
+Qed.
+
+Lemma prop_solve_eq_spec x:
+  to_prop'' x ->
+  to_prop'' (prop_solve_eq x).
+Proof.
+  destruct x as [x0 x1].
+  unfold to_prop''.
+  intros H mp.
+  cbn.
+  specialize (H mp).
+  cbn in H.
+  pose proof (solve_eqs_spec mp mpi x0).
+  tauto.
+Qed.
+
+
+Lemma try_subst_spec cfg x i:
+  let '((x',i'),_):=(TrySubst.try_subst cfg x i) in
+  (to_prop'' x) -> (to_prop'' x').
+Proof.
+  destruct x as [H G].
+  cbn.
+  destruct (TrySubst.list_find_subst cfg H (PositiveMap.empty expr_expr, PositiveMap.empty unit, i)) as [[sl _] _].
+  intros H0.
+  apply (subst_spec (H,G)),H0.
+Qed.
+
+Lemma solve_assumptions_spec n cfg x i:
+to_prop'' x ->
+match solve_assumptions n cfg x i with
+| None => True
+| Some (x',_) => to_prop'' x'
+end.
+Proof.
+  gen x i.
+  induction n; intros x i H.
+  1: cbn; trivial.
+  cbn.
+  destruct (prop_has_false (prop_solve_eq x)).
+  1: trivial.
+  pose proof (prop_solve_eq_spec x H) as H0.
+  pose proof (try_subst_spec cfg (prop_solve_eq x) i) as H1.
+  destruct (TrySubst.try_subst cfg (prop_solve_eq x) i) as [[x0 i0] mp0].
+  specialize (H1 H0).
+  destruct (list_prop0_eqb (fst x0) []).
+  1: tauto.
+  destruct (prop_eqb x0 x).
+  1: trivial.
+  specialize (IHn x0 i0 H1).
+  destruct (solve_assumptions n cfg x0 i0) as [[]|]; trivial.
+Qed.
+
+Lemma rename_var_by_sort_spec x:
+  to_prop'' x ->
+  to_prop'' (fst (rename_var_by_sort x)).
+Proof.
+  unfold rename_var_by_sort.
+  destruct (prop_allFV x S0) as [f p].
+  cbn.
+  apply subst_spec.
+Qed.
+
+Lemma prop_simpl_spec' x:
+  to_prop'' x -> to_prop'' (SimplExpr.simpl_prop x).
+Proof.
+  unfold to_prop''.
+  intros H mp.
+  rewrite prop_simpl_spec.
+  apply H.
+Qed.
+
+Lemma simpl_rule_spec x:
+  to_prop'' x ->
+  to_prop'' (fst (simpl_rule x)).
+Proof.
+  intro H3.
+  apply rename_var_by_sort_spec.
+  apply prop_simpl_spec'.
+  apply H3.
+Qed.
+
+Lemma follow_rule_spec w1 w2:
+to_prop'' (fst w1) ->
+to_prop'' (fst w2) ->
+match follow_rule w1 w2 with
+| None => True
+| Some w =>
+  to_prop'' (fst w)
+end.
+Proof.
+  destruct w1 as [x1 i1].
+  destruct w2 as [x2 i2].
+  cbn.
+  intros H1 H2.
+  pose proof (prop_merge_spec x1 x2 i1 H1 H2) as H.
+  destruct_spec prop_multistep'_trans_spec. 2: tauto.
+  destruct_spec solve_assumptions_spec; trivial.
+  destruct p0.
+  apply simpl_rule_spec. tauto.
+Qed.
+
+Transparent solve_assumptions_iter_limit.
+
+
+
+
+Lemma solve_apply_spec w1 w2:
+  to_prop'' (fst w1) ->
+  solve_apply w1 w2 = true ->
+  to_prop'' (fst w2).
+Proof.
+  unfold to_prop'',solve_apply.
+  intros H H0 mp.
+  destruct (subst_for_apply w1 w2); try congruence.
+  rewrite <-ExprEq_prop_spec.
+  2: apply H0.
+  apply subst_spec.
+  unfold to_prop''.
+  apply H.
+Qed.
+
+End ivar.
+
+
+
+Section fext.
+Hypothesis mp mp': (id_t -> forall t : type_t, to_type t).
+Hypothesis mpi: N.
+Hypothesis mp_eq: forall i t, mp i t = mp' i t.
+
+Lemma to_nat_fext x:
+  to_nat mp mpi x = to_nat mp' mpi x.
+Proof.
+  induction x; cbn.
+  all: congruence.
+Qed.
+
+Lemma to_seg_fext x:
+  to_seg mp mpi x = to_seg mp' mpi x.
+Proof.
+  induction x; cbn.
+  all: repeat rewrite to_nat_fext; congruence.
+Qed.
+
+Lemma to_side_fext x:
+  to_side mp mpi x = to_side mp' mpi x.
+Proof.
+  induction x; cbn.
+  all: repeat rewrite to_seg_fext; repeat rewrite to_nat_fext; congruence.
+Qed.
+
+Lemma to_config_fext x:
+  to_config mp mpi x = to_config mp' mpi x.
+Proof.
+  destruct x as [[[l r] s] sgn]; cbn.
+  repeat rewrite to_side_fext.
+  reflexivity.
+Qed.
+
+Lemma to_prop0_fext x:
+  to_prop0 mp mpi x = to_prop0 mp' mpi x.
+Proof.
+  destruct x; cbn.
+  all: repeat rewrite to_nat_fext.
+  all: repeat rewrite to_seg_fext.
+  all: repeat rewrite to_side_fext.
+  all: repeat rewrite to_config_fext.
+  all: congruence.
+Qed.
+
+Lemma to_prop0_list_fext x:
+  to_prop0_list mp mpi x <-> to_prop0_list mp' mpi x.
+Proof.
+  unfold to_prop0_list.
+  induction x; cbn.
+  all: repeat rewrite Forall_nil_iff.
+  all: repeat rewrite Forall_cons_iff.
+  all: repeat rewrite to_prop0_fext.
+  all: tauto.
+Qed.
+
+Lemma to_prop_fext x:
+  to_prop mp mpi x <-> to_prop mp' mpi x.
+Proof.
+  destruct x as [H G]. cbn.
+  repeat rewrite to_prop0_list_fext.
+  tauto.
+Qed.
+End fext.
+
+Definition to_prop' x :=
+  forall mpi, to_prop'' mpi x.
+
+Lemma follow_rule_spec' w1 w2:
+  to_prop' (fst w1) ->
+  to_prop' (fst w2) ->
+  match follow_rule w1 w2 with
+  | Some w => to_prop' (fst w)
+  | None => True
+  end.
+Proof.
+  intros H1 H2.
+  destruct (follow_rule w1 w2) eqn:E; trivial.
+  intros mpi.
+  pose proof (follow_rule_spec mpi w1 w2) as H.
+  rewrite E in H.
+  apply H.
+  - apply H1.
+  - apply H2.
+Qed.
+
+Lemma subst_ivar_spec w n n0:
+  to_prop'' n (SubstExpr.subst_prop subst_identity n0 w) ->
+  forall mp, to_prop mp (to_nat mp n n0) w.
+Proof.
+  intros H mp.
+  specialize (H mp).
+  rewrite (prop_subst_spec) in H.
+  cbn in H.
+  unfold subst_identity in H.
+  unfold tm_ctx.mp in H.
+  erewrite to_prop_fext.
+  - apply H.
+  - intros.
+    destruct t;
+    reflexivity.
+Qed.
+
+Lemma solve_ind_spec (wO wS w:prop_expr'):
+  (to_prop' (fst wO)) ->
+  (to_prop' (fst wS)) ->
+  solve_ind wO wS w = true ->
+  (to_prop' (fst w)).
+Proof.
+  intros HO HS H n.
+  unfold solve_ind in H.
+  induction n using N.peano_ind; intros.
+  - eassert (forall i:N, _) as X. {
+      intro i.
+      pose proof (follow_rule_spec i w wS) as H0.
+      destruct (follow_rule w wS) as [w'|]; try congruence.
+      rewrite and_true_iff in H.
+      destruct H as [Ha Hb].
+      eapply (solve_apply_spec i wO _ (HO i) Ha).
+    }
+    cbn in X.
+    intro mp.
+    apply (subst_ivar_spec _ _ _ (X N0) mp).
+  - eassert (_) as X. {
+      pose proof (follow_rule_spec n w wS) as H0.
+      destruct (follow_rule w wS) as [w'|]; try congruence.
+      rewrite and_true_iff in H.
+      destruct H as [Ha Hb].
+      eapply (solve_apply_spec n w' _ _ Hb).
+    Unshelve.
+      apply (H0).
+      - apply IHn.
+      - apply HS.
+    }
+    cbn in X.
+    intro mp.
+    replace (N.succ n) with (n+1)%N by lia.
+    apply (subst_ivar_spec _ _ _ X mp).
+Qed.
+
+
+
+
+
+Lemma remove_ivar_spec x:
+  to_prop' (fst x) ->
+  to_prop' (fst (remove_ivar x)).
+Proof.
+  destruct x as [x0 i]; cbn.
+  intros H n.
+  apply simpl_rule_spec.
+  intros mp.
+  rewrite prop_subst_spec.
+  rewrite to_prop_fext.
+  1: apply (H _ mp).
+  intros i0 t.
+  destruct t;
+  reflexivity.
+Qed.
+
+Lemma specialize_ivar_spec x n:
+  to_prop' (fst x) ->
+  to_prop' (fst (specialize_ivar x n)).
+Proof.
+  destruct x as [x0 i]; cbn.
+  intros H n0.
+  apply simpl_rule_spec.
+  intros mp.
+  rewrite prop_subst_spec.
+  rewrite to_prop_fext.
+  1: apply (H _ mp).
+  intros i0 t.
+  destruct t;
+  reflexivity.
+Qed.
+
+Lemma step0_refl_spec s sgn:
+  to_prop' (fst (step0_refl s sgn)).
+Proof.
+  intros mp mpi.
+  cbn.
+  unfold to_prop0_list.
+  repeat rewrite Forall_cons_iff.
+  repeat rewrite Forall_nil_iff.
+  cbn.
+  destruct sgn; cbn;
+  intro; split; trivial.
+Qed.
+
+Lemma find_step0_refl_spec x:
+  match find_step0_refl x with
+  | None => True
+  | Some x0 => to_prop' (fst x0)
+  end.
+Proof.
+  unfold find_step0_refl.
+  destruct (get_config_r x) as [[[[l r] s] sgn]|]; trivial.
+  apply step0_refl_spec.
+Qed.
+
+Lemma multistep'_for_ind_spec w:
+  to_prop' (fst w) ->
+  to_prop' (fst (multistep'_for_ind w)).
+Proof.
+  destruct w as [[H G] i].
+  destruct G as [|G0 G]; cbn.
+  1: tauto.
+  destruct G0; cbn; try tauto.
+  destruct n; cbn; try tauto.
+  intros H0 mpi mp.
+  specialize (H0 mpi mp).
+  gen H0.
+  cbn.
+  unfold to_prop0_list.
+  repeat rewrite Forall_cons_iff.
+  cbn.
+  intros H0 H1.
+  specialize (H0 H1).
+  split; try tauto.
+  apply progress_evstep. tauto.
+Qed.
+
+Lemma step1_to_step0_spec w:
+  to_prop' (fst w) ->
+  to_prop' (fst (step1_to_step0 w)).
+Proof.
+  destruct w as [[H G] i].
+  destruct G as [|[] G]; try tauto.
+  destruct n; try tauto.
+  cbn.
+  unfold to_prop'.
+  intros H0 mpi mp.
+  specialize (H0 mpi mp).
+  gen H0.
+  unfold to_prop,to_prop0_list.
+  repeat rewrite Forall_cons_iff.
+  intros H1 H2.
+  specialize (H1 H2).
+  destruct H1 as [H1 H3].
+  split; try tauto.
+  gen H1.
+  cbn.
+  apply progress_evstep.
+Qed.
+
+Lemma subst_ind_S_spec w mp:
+  to_prop' (fst w) ->
+  to_prop' (fst (subst_ind_S w mp)).
+Proof.
+  intro H.
+  cbn.
+  intros mpi.
+  apply subst_spec.
+  apply step1_to_step0_spec,H.
+Qed.
+
+Lemma solve_apply_spec' w1 w2:
+  to_prop' (fst w1) ->
+  if solve_apply w1 w2 then to_prop' (fst w2)
+  else True.
+Proof.
+  pose proof (fun mpi => solve_apply_spec mpi w1 w2).
+  destruct (solve_apply w1 w2); trivial.
+  intros H' mpi.
+  apply H; trivial.
+Qed.
+
+Lemma try_ind_spec w1 w0' w0:
+  to_prop' (fst w1) ->
+  to_prop' (fst w0') ->
+  match try_ind w1 w0' w0 with
+  | None => True
+  | Some (x,x0) => to_prop' (fst x) /\ to_prop' (fst x0)
+  end.
+Proof.
+  intros H' H0'.
+  unfold try_ind.
+  destruct w1 as [x1 i1].
+  destruct (FindIH.find_IH x1 i1 (fst w0') (fst w0)) as [[[[x2 x3] mp] n]|]; trivial.
+  destruct_spec find_step0_refl_spec; trivial.
+  destruct_spec solve_ind_spec; trivial.
+  assert (to_prop' (fst x2)) as H1. {
+    unfold to_prop'.
+    apply H0; trivial.
+    apply subst_ind_S_spec. tauto.
+  }
+  destruct n as [n|].
+  - destruct_spec solve_apply_spec'; trivial.
+    destruct_spec follow_rule_spec'; trivial.
+    destruct_spec follow_rule_spec'; trivial.
+    split.
+    + apply remove_ivar_spec. tauto.
+    + apply H4; try tauto.
+      apply specialize_ivar_spec. tauto.
+  - destruct_spec follow_rule_spec'; trivial.
+    split.
+    + apply remove_ivar_spec,H1.
+    + apply H2; try tauto.
+      apply remove_ivar_spec,H1.
+Qed.
+
+
+
+
+
+
+
+
+
+Definition to_prop0' x :=
+  forall mp mpi, to_prop0 mp mpi x.
+
+Definition side_0inf_def:=
+  (side_eq
+  side_0inf
+  (side_concat (seg_sym s0) side_0inf),
+  1%positive).
+
+Lemma side_0inf_def_spec:
+  to_prop0' (fst (side_0inf_def)).
+Proof.
+  unfold to_prop0'.
+  intros. cbn.
+  rewrite <-const_unfold.
+  reflexivity.
+Qed.
+
+
+Fixpoint side_concat_unfold(r0:seg_expr)(r:side_expr):side_expr :=
+match r0 with
+| seg_concat r1 r2 =>
+  side_concat r1 (side_concat_unfold r2 r)
+| _ => side_concat r0 r
+end.
+
+Lemma side_concat_unfold_spec r0 r mp mpi:
+  to_side mp mpi (side_concat_unfold r0 r) =
+  to_seg mp mpi r0 *> to_side mp mpi r.
+Proof.
+  induction r0; try reflexivity.
+  cbn.
+  rewrite IHr0_2,Str_app_assoc.
+  reflexivity.
+Qed.
+
+Definition repeat_S_def(r0:seg_expr):=
+  let n:=nat_var 1%positive in
+  let r:=side_var 2%positive in
+  (side_eq
+  (side_concat (seg_repeat r0 (nat_add n (from_nat 1))) r)
+  (side_concat_unfold r0 (side_concat (seg_repeat r0 n) r)),
+  3%positive).
+
+Lemma repeat_S_def_spec r0:
+  to_prop0' (fst (repeat_S_def r0)).
+Proof.
+  unfold to_prop0'.
+  intros.
+  cbn.
+  rewrite N.add_comm.
+  rewrite Nnat.N2Nat.inj_add.
+  rewrite lpow_add.
+  rewrite Str_app_assoc.
+  change (N.to_nat 1) with 1.
+  cbn.
+  rewrite List.app_nil_r.
+  rewrite side_concat_unfold_spec.
+  reflexivity.
+Qed.
+
+Definition repeat_2_def(r0:seg_expr):=
+  let r:=side_var 1%positive in
+  (side_eq
+  (side_concat (seg_repeat r0 (from_nat 2)) r)
+  (side_concat_unfold r0 (side_concat_unfold r0 r)),
+  2%positive).
+
+Lemma repeat_2_def_spec r0:
+  to_prop0' (fst (repeat_2_def r0)).
+Proof.
+  unfold to_prop0'.
+  intros.
+  cbn.
+  change (Pos.to_nat 2) with 2.
+  cbn.
+  repeat rewrite Str_app_assoc.
+  cbn.
+  do 2 rewrite side_concat_unfold_spec.
+  reflexivity.
+Qed.
+
+Definition repeat_0_def(r0:seg_expr):=
+  let r:=side_var 1%positive in
+  (side_eq
+  (side_concat (seg_repeat r0 (from_nat 0)) r)
+  r,
+  2%positive).
+
+Lemma repeat_0_def_spec r0:
+  to_prop0' (fst (repeat_0_def r0)).
+Proof.
+  unfold to_prop0'.
+  reflexivity.
+Qed.
+
+Definition repeat_0_def'(r0:seg_expr):=
+  let r:=side_var 1%positive in
+  (side_eq
+  r
+  (side_concat (seg_repeat r0 (from_nat 0)) r),
+  2%positive).
+
+Lemma repeat_0_def_spec' r0:
+  to_prop0' (fst (repeat_0_def' r0)).
+Proof.
+  unfold to_prop0'.
+  reflexivity.
+Qed.
+
+Definition step1 m s sgn :=
+  let l:=side_var 1%positive in
+  let r:=side_var 2%positive in
+  match tm (s,m) with
+  | None => None
+  | Some (m',sgn',s') =>
+    Some (
+    if dir_eqb sgn sgn' then
+      (multistep'_expr
+      (l,side_concat (seg_sym m) r,s,sgn)
+      (side_concat (seg_sym m') l,r,s',sgn)
+      true,
+      3%positive)
+    else
+      (multistep'_expr
+      (l,side_concat (seg_sym m) r,s,sgn)
+      (side_concat (seg_sym m') r,l,s',sgn')
+      true,
+      3%positive))
+  end.
+
+Lemma step1_spec m s sgn:
+  match step1 m s sgn with
+  | None => True
+  | Some x => to_prop0' (fst x)
+  end.
+Proof.
+  unfold step1.
+  destruct (tm (s,m)) as [[[m' sgn'] s']|] eqn:E.
+  2: trivial.
+  destruct sgn,sgn'; unfold to_prop0'; intros; cbn.
+  all: apply progress_base; constructor; apply E.
+Qed.
+
+Fixpoint side_find_repeat_2_fold(ls1 ls2:side_expr)(n:nat):=
+match n with
+| O =>
+  match ls1,ls2 with
+  | side_concat h1 t1,side_concat h2 t2 =>
+    if seg_expr_eqb h1 h2 then Some h1 else None
+  | _,_ => None
+  end
+| Datatypes.S n0 =>
+  match ls1,ls2 with
+  | side_concat h1 t1,side_concat h2 t2 =>
+    if seg_expr_eqb h1 h2 then
+      match side_find_repeat_2_fold t1 t2 n0 with
+      | Some v => Some (seg_concat h1 v)
+      | None => None
+      end
+    else None
+  | _,_ => None
+  end
+end.
+
+Fixpoint side_check_repeat_S_fold(ls1:side_expr)(ls2:seg_expr)(n:nat):=
+match n with
+| O =>
+  match ls1 with
+  | side_concat h1 t1 => seg_expr_eqb h1 ls2
+  | _ => false
+  end
+| Datatypes.S n0 =>
+  match ls1,ls2 with
+  | side_concat h1 t1,seg_concat h2 t2 =>
+     seg_expr_eqb h1 h2 && side_check_repeat_S_fold t1 t2 n0
+  | _,_ => false
+  end
+end.
+
+Definition side_find_repeat_S_fold ls1 ls2 n :=
+match ls2 with
+| side_concat (seg_repeat h2 _) _ =>
+  if side_check_repeat_S_fold ls1 h2 n then Some h2 else None
+| _ => None
+end.
+
+Definition side_find_repeat_O_fold ls :=
+match ls with
+| side_concat (seg_repeat h (from_nat 0)) _ => Some h
+| _ => None
+end.
+
+Definition side_find_repeat_fold_1 ls1 ls2 n :=
+match side_find_repeat_2_fold ls1 ls2 n with
+| Some h => Some (repeat_2_def h)
+| None =>
+  match side_find_repeat_S_fold ls1 ls2 n with
+  | Some h => Some (repeat_S_def h)
+  | None => None
+  end
+end.
+
+Fixpoint side_find_repeat_fold_2 ls1 ls2 n n0 {struct n0} :=
+match n0 with
+| O => None
+| Datatypes.S n1 =>
+  match
+    match n with
+    | Datatypes.S n2 => side_find_repeat_fold_1 ls1 ls2 n2
+    | O => None
+    end
+  with
+  | Some h => Some h
+  | None =>
+    match ls2 with
+    | side_concat h2 t2 =>
+      side_find_repeat_fold_2 ls1 t2 (Datatypes.S n) n1
+    | _ => None
+    end
+  end
+end.
+
+Definition side_concat_rw_2(x:prop0_expr*id_t):prop0_expr*id_t :=
+match x with
+| (side_eq a b,p) =>
+  let (v,p):=(seg_var p,Pos.succ p) in
+  (side_eq (side_concat v a) (side_concat v b),p)
+| _ => x
+end.
+
+Lemma side_concat_rw_2_spec x:
+  to_prop0' (fst x) ->
+  to_prop0' (fst (side_concat_rw_2 x)).
+Proof.
+  unfold to_prop0'.
+  destruct x as [x i].
+  cbn.
+  intros H mp mpi.
+  specialize (H mp mpi).
+  destruct x; cbn; cbn in H; congruence.
+Qed.
+
+Definition max_repeater_len:nat := 8.
+
+Fixpoint side_find_repeat_fold ls1 :=
+match side_find_repeat_O_fold ls1 with
+| Some h => Some (repeat_0_def' h)
+| None =>
+  match ls1 with
+  | side_concat h1 t1 =>
+    match side_find_repeat_fold t1 with
+    | Some v => Some (side_concat_rw_2 v)
+    | None =>
+      match side_find_repeat_fold_2 ls1 ls1 O max_repeater_len with
+      | Some v => Some v
+      | None => None
+      end
+    end
+  | _ => None
+  end
+end.
+
+Opaque max_repeater_len.
+
+Lemma side_find_repeat_fold_1_spec ls1 ls2 n:
+  match side_find_repeat_fold_1 ls1 ls2 n with
+  | None => True
+  | Some x => to_prop0' (fst x)
+  end.
+Proof.
+  unfold side_find_repeat_fold_1.
+  destruct (side_find_repeat_2_fold ls1 ls2 n).
+  1: apply repeat_2_def_spec.
+  destruct (side_find_repeat_S_fold ls1 ls2 n).
+  1: apply repeat_S_def_spec.
+  trivial.
+Qed.
+
+
+Lemma side_find_repeat_fold_2_spec ls1 ls2 n n0:
+  match side_find_repeat_fold_2 ls1 ls2 n n0 with
+  | None => True
+  | Some x => to_prop0' (fst x)
+  end.
+Proof.
+  gen ls2 n.
+  induction n0; cbn; intros; trivial.
+  destruct n as [|n]; cbn.
+  - destruct ls2; cbn; trivial.
+    apply IHn0.
+  - pose proof (side_find_repeat_fold_1_spec ls1 ls2 n) as H.
+    destruct (side_find_repeat_fold_1 ls1 ls2 n); try tauto.
+    destruct ls2; cbn; trivial.
+    apply IHn0.
+Qed.
+
+Lemma side_find_repeat_fold_spec ls:
+  match side_find_repeat_fold ls with
+  | None => True
+  | Some x => to_prop0' (fst x)
+  end.
+Proof.
+  induction ls.
+  1,2: cbn; trivial.
+  cbn[side_find_repeat_fold].
+  destruct (side_find_repeat_O_fold (side_concat a ls)).
+  1: apply repeat_0_def_spec'.
+  destruct (side_find_repeat_fold ls).
+  - apply side_concat_rw_2_spec,IHls.
+  - pose proof (side_find_repeat_fold_2_spec (side_concat a ls) (side_concat a ls) 0 max_repeater_len).
+    destruct (side_find_repeat_fold_2 (side_concat a ls) (side_concat a ls) 0 max_repeater_len); tauto.
+Qed.
+
+Transparent max_repeater_len.
+
+Definition config_rw_l(x:prop0_expr*id_t) s sgn:prop0_expr*id_t :=
+match x with
+| (side_eq l1 l2,p) =>
+  let (r,p):=(side_var p,Pos.succ p) in 
+  (config_eq (l1,r,s,sgn) (l2,r,s,sgn),p)
+| _ => x
+end.
+
+Definition config_rw_r(x:prop0_expr*id_t) s sgn:prop0_expr*id_t :=
+match x with
+| (side_eq r1 r2,p) =>
+  let (l,p):=(side_var p,Pos.succ p) in 
+  (config_eq (l,r1,s,sgn) (l,r2,s,sgn),p)
+| _ => x
+end.
+
+Lemma config_rw_l_spec x s sgn:
+  to_prop0' (fst x) ->
+  to_prop0' (fst (config_rw_l x s sgn)).
+Proof.
+  unfold to_prop0'.
+  destruct x as [x i]; cbn.
+  intros H mp.
+  specialize (H mp).
+  destruct x,sgn; cbn; cbn in H; try tauto; congruence.
+Qed.
+
+Lemma config_rw_r_spec x s sgn:
+  to_prop0' (fst x) ->
+  to_prop0' (fst (config_rw_r x s sgn)).
+Proof.
+  unfold to_prop0'.
+  destruct x as [x i]; cbn.
+  intros H mp.
+  specialize (H mp).
+  destruct x,sgn; cbn; cbn in H; try tauto; congruence.
+Qed.
+
+Definition config_find_repeat_fold(c:config_expr) :=
+let '(l,r,s,sgn):=c in
+match side_find_repeat_fold l with
+| Some x => Some (config_rw_l x s sgn)
+| None =>
+  match side_find_repeat_fold r with
+  | Some x => Some (config_rw_r x s sgn)
+  | None => None
+  end
+end.
+
+Lemma config_find_repeat_fold_spec c:
+  match config_find_repeat_fold c with
+  | None => True
+  | Some x => to_prop0' (fst x)
+  end.
+Proof.
+  destruct c as [[[l r] s] sgn]; cbn.
+  pose proof (side_find_repeat_fold_spec l) as H.
+  destruct (side_find_repeat_fold l).
+  1: apply config_rw_l_spec,H.
+  pose proof (side_find_repeat_fold_spec r) as H0.
+  destruct (side_find_repeat_fold r).
+  1: apply config_rw_r_spec,H0.
+  trivial.
+Qed.
+
+
+
+Definition side_find_repeat_unfold ls :=
+match ls with
+| side_0inf => Some side_0inf_def
+| side_concat (seg_repeat a (from_nat 0)) r => Some (repeat_0_def a)
+| side_concat (seg_repeat a _) r => Some (repeat_S_def a)
+| _ => None
+end.
+
+Lemma side_find_repeat_unfold_spec ls:
+  match side_find_repeat_unfold ls with
+  | None => True
+  | Some x => to_prop0' (fst x)
+  end.
+Proof.
+  destruct ls; cbn; trivial.
+  - apply side_0inf_def_spec.
+  - destruct a; trivial.
+    destruct n.
+    1: destruct n.
+    all: try (apply repeat_S_def_spec).
+    apply repeat_0_def_spec.
+Qed.
+
+Definition config_find_repeat_unfold(c:config_expr) :=
+let '(l,r,s,sgn):=c in
+  match side_find_repeat_unfold r with
+  | Some x => Some (config_rw_r x s sgn)
+  | None => None
+  end.
+
+Lemma config_find_repeat_unfold_spec c:
+  match config_find_repeat_unfold c with
+  | None => True
+  | Some x => to_prop0' (fst x)
+  end.
+Proof.
+  destruct c as [[[l r] s] sgn].
+  cbn.
+  pose proof (side_find_repeat_unfold_spec r) as H.
+  destruct (side_find_repeat_unfold r); trivial.
+  apply config_rw_r_spec,H.
+Qed.
+
+Definition step0_rw_l(x:prop0_expr*id_t) :=
+match x with
+| (config_eq c1 c2,p) =>
+  (multistep'_expr c2 c1 false,p)
+| _ => x
+end.
+
+Definition step0_rw_r(x:prop0_expr*id_t) :=
+match x with
+| (config_eq c1 c2,p) =>
+  (multistep'_expr c1 c2 false,p)
+| _ => x
+end.
+
+Lemma step0_rw_l_spec x:
+  to_prop0' (fst x) ->
+  to_prop0' (fst (step0_rw_l x)).
+Proof.
+  unfold to_prop0'.
+  destruct x as [x i].
+  cbn.
+  intros H mp mpi.
+  specialize (H mp mpi).
+  destruct x; cbn; cbn in H; try tauto.
+  rewrite H.
+  constructor.
+Qed.
+
+Lemma step0_rw_r_spec x:
+  to_prop0' (fst x) ->
+  to_prop0' (fst (step0_rw_r x)).
+Proof.
+  unfold to_prop0'.
+  destruct x as [x i].
+  cbn.
+  intros H mp mpi.
+  specialize (H mp mpi).
+  destruct x; cbn; cbn in H; try tauto.
+  rewrite H.
+  constructor.
+Qed.
+
+
+
+Definition prop0_to_prop(x:prop0_expr*id_t):prop_expr' :=
+let (x,i):=x in
+(([],[x]),i).
+
+Definition next_rule f x :=
+match get_config_r x with
+| None => None
+| Some c =>
+  match f c with
+  | None => None
+  | Some x0 => Some (prop0_to_prop x0)
+  end
+end.
+
+Lemma prop0_to_prop_spec x:
+  to_prop0' (fst x) ->
+  to_prop' (fst (prop0_to_prop x)).
+Proof.
+  destruct x as [x i]; cbn.
+  intros H mpi mp.
+  specialize (H mp mpi).
+  cbn.
+  unfold to_prop0_list.
+  repeat rewrite Forall_cons_iff.
+  repeat rewrite Forall_nil_iff.
+  tauto.
+Qed.
+
+Lemma next_rule_spec f x:
+  (forall c,
+  match f c with
+  | None => True
+  | Some x => to_prop0' (fst x)
+  end) ->
+  to_prop' (fst x) ->
+  match next_rule f x with
+  | None => True
+  | Some x0 => to_prop' (fst x0)
+  end.
+Proof.
+  intros H0 H.
+  unfold next_rule.
+  destruct (get_config_r x); trivial.
+  specialize (H0 c).
+  destruct (f c); trivial.
+  apply prop0_to_prop_spec,H0.
+Qed.
+
+Definition hlin_layer:Type := (prop_expr'*prop_expr')*(prop_expr'*prop_expr')*(N*N).
+
+Definition hlin_layer_WF(x:hlin_layer):Prop :=
+  let '((w1_,w0_),(w1,w0),_):=x in
+  to_prop' (fst w1_) /\
+  to_prop' (fst w0_) /\
+  to_prop' (fst w1) /\
+  to_prop' (fst w0).
+
+Definition hlin_layers_WF(x:list hlin_layer):Prop :=
+  Forall hlin_layer_WF x.
+
+Definition step0_refl' x :=
+match find_step0_refl x with
+| None => x
+| Some x => x
+end.
+
+Lemma step0_refl'_spec x:
+  to_prop' (fst x) ->
+  to_prop' (fst (step0_refl' x)).
+Proof.
+  unfold step0_refl'.
+  pose proof (find_step0_refl_spec x).
+  destruct (find_step0_refl x); tauto.
+Qed.
+
+Definition reset_hlin_layers u0 :=
+((step0_refl' u0,u0),(step0_refl' u0,u0),(1,2)%N)::nil.
+
+Lemma reset_hlin_layers_spec x:
+  to_prop' (fst x) ->
+  hlin_layers_WF (reset_hlin_layers x).
+Proof.
+  intro H.
+  unfold hlin_layers_WF,reset_hlin_layers.
+  apply Forall_cons; auto.
+  cbn.
+  repeat split; auto using step0_refl'_spec.
+Qed.
+
+Definition get_w0(ls:list hlin_layer)(u:prop_expr') :=
+match ls with
+| (_,(_,w0),_)::ls => w0
+| _ => u
+end.
+
+Lemma get_w0_spec ls u :
+  hlin_layers_WF ls ->
+  to_prop' (fst u) ->
+  to_prop' (fst (get_w0 ls u)).
+Proof.
+  destruct ls; cbn.
+  1: tauto.
+  destruct h as [[[w1_ w0_] [w1 w0]] [l r]]; cbn.
+  unfold hlin_layers_WF.
+  rewrite Forall_cons_iff; cbn.
+  tauto.
+Qed.
+
+(*
+  u1: Q2 --> Q3
+  u0: c0 --> P := w0 u1
+
+  w1_: Q0 --> Q1
+  w1: Q1 --> Q2
+  w0 := w0_ w1
+*)
+Fixpoint hlin_layers_upd(u1 u0:prop_expr')(ls:list hlin_layer): (list hlin_layer) :=
+let u := (reset_hlin_layers u0) in
+match ls with
+| nil => u
+| w::ls =>
+  let '((w1_,w0_),(w1,_),(l,r)) := w in
+  match follow_rule w1 u1 with
+  | None => u
+  | Some w1' =>
+    match try_ind w1' w0_ u0 with
+    | Some (u1',u0') =>
+      match follow_rule w1_ u1' with
+      | None => reset_hlin_layers u1'
+      | Some w1'' =>
+        let ls':=hlin_layers_upd w1'' u0' ls in
+        let u0'':= get_w0 ls' u0' in
+        ((step0_refl' u0'',u0''),(step0_refl' u0'',u0''),(1,2)%N)::
+        ls'
+      end
+    | None =>
+      let l := N.succ l in
+      if (l<?r)%N then
+        ((w1_,w0_),(w1',u0),(l,r))::ls
+      else
+        match follow_rule w1_ w1' with
+        | None => u
+        | Some w1_ =>
+          ((w1_,u0),(step0_refl' u0,u0),(l,r*2)%N)::ls
+        end
+    end
+  end
+end.
+
+Lemma hlin_layers_upd_spec u1 u0 ls:
+  to_prop' (fst u1) ->
+  to_prop' (fst u0) ->
+  hlin_layers_WF ls ->
+  hlin_layers_WF (hlin_layers_upd u1 u0 ls).
+Proof.
+  gen u1 u0.
+  induction ls; introv H1 H0 H.
+  1: apply reset_hlin_layers_spec,H0.
+  unfold hlin_layers_WF in H.
+  rewrite Forall_cons_iff in H.
+  destruct H as [Ha Hls].
+  destruct a as [[[w1_ w0_] [w1 w0]] [l r]].
+  cbn in Ha.
+  cbn.
+  pose proof (follow_rule_spec' w1 u1).
+  destruct (follow_rule w1 u1) as [w1'|].
+  2: apply reset_hlin_layers_spec; tauto.
+  pose proof (try_ind_spec w1' w0_ u0).
+  destruct (try_ind w1' w0_ u0) as [[u1' u0']|].
+  - pose proof (follow_rule_spec' w1_ u1').
+    destruct (follow_rule w1_ u1').
+    2: apply reset_hlin_layers_spec; try tauto.
+    unfold hlin_layers_WF.
+    apply Forall_cons.
+    2: apply IHls; tauto.
+    cbn.
+    epose proof (get_w0_spec (hlin_layers_upd p u0' ls) u0' _ _).
+    pose proof (step0_refl'_spec (get_w0 (hlin_layers_upd p u0' ls) u0')).
+    repeat split; tauto.
+    Unshelve.
+      2: tauto.
+      apply IHls; tauto.
+  - destruct (N.succ l <? r)%N.
+    + unfold hlin_layers_WF.
+      apply Forall_cons; try tauto.
+      cbn.
+      repeat split; tauto.
+    + pose proof (follow_rule_spec' w1_ w1').
+      destruct (follow_rule w1_ w1').
+      2: apply reset_hlin_layers_spec; tauto.
+      unfold hlin_layers_WF.
+      apply Forall_cons; try tauto.
+      cbn.
+      pose proof (step0_refl'_spec u0).
+      repeat split; tauto.
+Qed.
+
+
+Definition find_repeat_unfold x :=
+match get_config_r x with
+| None => None
+| Some x =>
+  match config_find_repeat_unfold x with
+  | None => None
+  | Some x =>
+    Some (prop0_to_prop (step0_rw_r x))
+  end
+end.
+
+Definition find_repeat_fold x :=
+match get_config_r x with
+| None => None
+| Some x =>
+  match config_find_repeat_fold x with
+  | None => None
+  | Some x =>
+    Some (prop0_to_prop (step0_rw_l x))
+  end
+end.
+
+Definition find_step1 x :=
+match get_config_r x with
+| None => None
+| Some x =>
+  let '(l,r,s,sgn):=x in
+  match r with
+  | side_concat (seg_sym m) r0 =>
+    match step1 m s sgn with
+    | None => None
+    | Some x0 => Some (prop0_to_prop x0)
+    end
+  | _ => None 
+  end
+end.
+
+Lemma find_repeat_unfold_spec x:
+to_prop' (fst x) ->
+match find_repeat_unfold x with
+| None => True
+| Some x =>
+  to_prop' (fst x)
+end.
+Proof.
+  intros H.
+  unfold find_repeat_unfold.
+  destruct (get_config_r x); trivial.
+  destruct_spec config_find_repeat_unfold_spec; trivial.
+  apply prop0_to_prop_spec.
+  apply step0_rw_r_spec,H0.
+Qed.
+
+Lemma find_repeat_fold_spec x:
+to_prop' (fst x) ->
+match find_repeat_fold x with
+| None => True
+| Some x =>
+  to_prop' (fst x)
+end.
+Proof.
+  intros H.
+  unfold find_repeat_fold.
+  destruct (get_config_r x); trivial.
+  destruct_spec config_find_repeat_fold_spec; trivial.
+  apply prop0_to_prop_spec.
+  apply step0_rw_l_spec,H0.
+Qed.
+
+Lemma find_step1_spec x:
+to_prop' (fst x) ->
+match find_step1 x with
+| None => True
+| Some x =>
+  to_prop' (fst x)
+end.
+Proof.
+  intros H.
+  unfold find_step1.
+  destruct (get_config_r x) as [[[[l r] s] sgn]|]; trivial.
+  destruct r; trivial.
+  destruct a; trivial.
+  destruct_spec step1_spec; trivial.
+  apply prop0_to_prop_spec,H0.
+Qed.
+
+
+Definition hlin_layers_upd' (ls:list hlin_layer)(f:prop_expr'->option prop_expr') :=
+match ls with
+| (_,(w1,w0),_)::_ =>
+  if (snd w0 =? 1)%positive then
+    match f w0 with
+    | None => None
+    | Some u1 =>
+      match follow_rule w0 u1 with
+      | None => None
+      | Some u0 =>
+        Some (hlin_layers_upd u1 u0 ls)
+      end
+    end
+  else None
+| _ => None
+end.
+
+Lemma hlin_layers_upd'_spec ls f:
+hlin_layers_WF ls ->
+(forall x,
+to_prop' (fst x) ->
+match f x with
+| None => True
+| Some x =>
+  to_prop' (fst x)
+end) ->
+match hlin_layers_upd' ls f with
+| None => True
+| Some ls' => hlin_layers_WF ls'
+end.
+Proof.
+  intros Hls Hf.
+  unfold hlin_layers_upd'.
+  destruct ls as [|[[[w1_ w0_] [w1 w0]] [l r]] ls0]; trivial.
+  destruct (snd w0 =? 1)%positive; trivial.
+  specialize (Hf w0).
+  pose proof Hls as Hls'.
+  unfold hlin_layers_WF in Hls.
+  rewrite Forall_cons_iff in Hls.
+  cbn in Hls.
+  destruct (f w0); trivial.
+  destruct_spec follow_rule_spec'; trivial.
+  apply hlin_layers_upd_spec; tauto.
+Qed.
+
+Fixpoint Pos_iter_until{S S'}(f:S->S+S')(x:S+S')(T:positive):S+S' :=
+match x with
+| inl s =>
+  match T with
+  | xH => f s
+  | xO T0 => Pos_iter_until f (Pos_iter_until f x T0) T0
+  | xI T0 => Pos_iter_until f (Pos_iter_until f (f s) T0) T0
+  end
+| _ => x
+end.
+
+Definition N_iter_until{S S'}(f:S->S+S')(x:S+S')(T:N):S+S' :=
+match T with
+| N0 => x
+| Npos T0 => Pos_iter_until f x T0
+end.
+
+
+Definition hlin_layers_step(s:(list hlin_layer)*bool):(list hlin_layer)*bool+(list hlin_layer) :=
+let (ls,o):=s in
+if o then
+  match hlin_layers_upd' ls find_step1 with
+  | None =>
+    match hlin_layers_upd' ls find_repeat_unfold with
+    | None => inr ls
+    | Some ls => inl (ls,true)
+    end
+  | Some ls =>
+    inl (ls,false)
+  end
+else
+  match hlin_layers_upd' ls find_repeat_fold with
+  | None => inl (ls,true)
+  | Some ls => inl (ls,false)
+  end.
+
+Definition step0_refl_c0:prop_expr' :=
+  ([],[multistep'_expr (side_0inf,side_0inf,q0,R) (side_0inf,side_0inf,q0,R) false],1%positive).
+
+Lemma step0_refl_c0_spec:
+  to_prop' (fst step0_refl_c0).
+Proof.
+  intros mpi mp.
+  cbn.
+  unfold to_prop0_list; cbn.
+  repeat rewrite Forall_cons_iff.
+  repeat rewrite Forall_nil_iff.
+  cbn.
+  intro; split; trivial.
+Qed.
+
+Definition hlin_layers_steps T :=
+N_iter_until hlin_layers_step (inl (reset_hlin_layers step0_refl_c0,true)) T.
+
+End tm_ctx.
+
+Declare Scope ind_scope.
+Delimit Scope ind_scope with ind.
+Bind Scope ind_scope with nat_expr.
+Bind Scope ind_scope with seg_expr.
+Bind Scope ind_scope with side_expr.
+Bind Scope ind_scope with config_expr.
+
+Notation "a *> b" := (side_concat a b) : ind_scope.
+Notation "a ; b" := (seg_concat a b) (at level 60, right associativity): ind_scope.
+Notation "a ^ b" := (seg_repeat a b) : ind_scope.
+Coercion seg_sym: Sym>->seg_expr.
+Notation "a + b" := (nat_add a b) : ind_scope.
+Notation "a * b" := (nat_mul a b) : ind_scope.
+Coercion from_nat: N>->nat_expr.
+Notation "'nv' a" := (nat_var a) (at level 35).
+Notation "'segv' a" := (seg_var a) (at level 35).
+Notation "'sv' a" := (side_var a) (at level 35).
+Notation "a -->* b" := (multistep'_expr a b false) (at level 40).
+Notation "a -->+ b" := (multistep'_expr a b true) (at level 40).
+Notation "'0...'" := side_0inf.
+
+
+(*
+config_find_repeat_unfold, step0_rw_r
+step1
+config_find_repeat_fold, step0_rw_l
+*)
+
+(*
+  (i i) (i i i)*
+  i+1 () ()
+*)
+
+
+
+
+(*
+(forall x, P(x,0)-->Q(x,0)) ->
+
+(forall n, (forall x, P(x,n)-->Q(x,n)) -> (forall x, P(x,n+1)-->Q(x,n+1))) ->
+
+(forall n, forall x, P(x,n)-->Q(x,n))
+*)
+
+
+
+
+(*
+prop_solve_eq: ((a,b)=(c,d) -> P) -> (a=c -> b=d -> P), also simpl nat affine map in H
+try_subst: (forall a, P(a)) -> forall a, P(f(a))
+prop_has_false: (False -> P) is trivial
+prop_eqb: check progress
+prop_merge: (A->B) -> (C->D) -> (A->C->(B/\D))
+simpl_prop: simpl nat affine map
+prop_multistep'_trans: (A-->B) -> (C-->D) -> (B=C -> A-->D)
+
+follow_rule: (A-->B) -> (B-->C) -> (A-->C)
+
+TODO WIP: induction
+TODO WIP: basic lemmas for TM execute and simpl tape
+*)
+
+End Inductive.
+
+
+
+
+
